zoo_saturn/inf_mpmc_queue_2: Rewrite.

theories/zoo_saturn/inf_mpmc_queue_2.v
@@ -34,9 +34,8 @@ From zoo Require Import
   options.
 
 Implicit Types b : bool.
-Implicit Types l : location.
 Implicit Types front back : nat.
-Implicit Types v t : val.
+Implicit Types v : val.
 Implicit Types o : option val.
 Implicit Types vs : list val.
 Implicit Types hist : list (option val).
@@ -220,343 +219,1336 @@ Proof.
   solve_inG.
 Qed.
 
+Module base.
+  Section inf_mpmc_queue_2_G.
+    Context `{inf_mpmc_queue_2_G : InfMpmcQueue2G Σ}.
+
+    Implicit Types t : location.
+    Implicit Types Ψ : val → iProp Σ.
+
+    Record inf_mpmc_queue_2_name := {
+      inf_mpmc_queue_2_name_data : val ;
+      inf_mpmc_queue_2_name_inv : namespace ;
+      inf_mpmc_queue_2_name_prophet : prophet_id ;
+      inf_mpmc_queue_2_name_prophet_name : wise_prophets_name ;
+      inf_mpmc_queue_2_name_model : gname ;
+      inf_mpmc_queue_2_name_history : gname ;
+      inf_mpmc_queue_2_name_lstates : gname ;
+      inf_mpmc_queue_2_name_producers : gname ;
+      inf_mpmc_queue_2_name_consumers : gname ;
+    }.
+    Implicit Type γ : inf_mpmc_queue_2_name.
+
+    #[global] Instance inf_mpmc_queue_2_name_eq_dec : EqDecision inf_mpmc_queue_2_name :=
+      ltac:(solve_decision).
+    #[global] Instance inf_mpmc_queue_2_name_countable :
+      Countable inf_mpmc_queue_2_name.
+    Proof.
+      solve_countable.
+    Qed.
+
+    #[local] Definition model₁' γ_model vs :=
+      twins_twin1 γ_model (DfracOwn 1) vs.
+    #[local] Definition model₁ γ vs :=
+      model₁' γ.(inf_mpmc_queue_2_name_model) vs.
+    #[local] Definition model₂' γ_model vs :=
+      twins_twin2 γ_model vs.
+    #[local] Definition model₂ γ vs :=
+      model₂' γ.(inf_mpmc_queue_2_name_model) vs.
+
+    #[local] Definition history_auth' γ_history hist :=
+      mono_list_auth γ_history (DfracOwn 1) hist.
+    #[local] Definition history_auth γ :=
+      history_auth' γ.(inf_mpmc_queue_2_name_history).
+    #[local] Definition history_at γ i o :=
+      mono_list_at γ.(inf_mpmc_queue_2_name_history) i o.
+
+    #[local] Definition lstates_auth' γ_lstates lstates : iProp Σ :=
+      ∃ ηs,
+      mono_list_auth γ_lstates (DfracOwn 1) ηs ∗
+      [∗ list] η; lstate ∈ ηs; lstates,
+        auth_mono_auth _ η DfracDiscarded lstate.
+    #[local] Definition lstates_auth γ :=
+      lstates_auth' γ.(inf_mpmc_queue_2_name_lstates).
+    #[local] Instance : CustomIpatFormat "lstates_auth" :=
+      " ( %ηs &
+          Hauth &
+          Hηs
+        )
+      ".
+    #[local] Definition lstates_at γ i lstate : iProp Σ :=
+      ∃ η,
+      mono_list_at γ.(inf_mpmc_queue_2_name_lstates) i η ∗
+      auth_mono_auth _ η DfracDiscarded lstate.
+    #[local] Instance : CustomIpatFormat "lstates_at" :=
+      " ( %η{} &
+          #Hat{_{}} &
+          #Hη_auth{_{}}
+        )
+      ".
+    #[local] Definition lstates_lb γ i lstate : iProp Σ :=
+      ∃ η,
+      mono_list_at γ.(inf_mpmc_queue_2_name_lstates) i η ∗
+      auth_mono_lb _ η lstate.
+    #[local] Instance : CustomIpatFormat "lstates_lb" :=
+      " ( %η{} &
+          #Hat{_{}} &
+          #Hη_lb{_{}}
+        )
+      ".
+
+    #[local] Definition producers_auth' γ_producers i : iProp Σ :=
+      ∃ ηs,
+      mono_list_auth γ_producers (DfracOwn 1) ηs ∗
+      ⌜length ηs = i⌝.
+    #[local] Definition producers_auth γ :=
+      producers_auth' γ.(inf_mpmc_queue_2_name_producers).
+    #[local] Instance : CustomIpatFormat "producers_auth" :=
+      " ( %ηs &
+          Hauth &
+          %Hηs
+        )
+      ".
+    #[local] Definition producers_at γ i own : iProp Σ :=
+      ∃ η,
+      mono_list_at γ.(inf_mpmc_queue_2_name_producers) i η ∗
+      match own with
+      | Own =>
+          oneshot_pending η (DfracOwn 1) ()
+      | Discard =>
+          oneshot_shot η ()
+      end.
+    #[local] Instance : CustomIpatFormat "producers_at" :=
+      " ( %η{} &
+          Hat{_{}} &
+          Hη{}
+        )
+      ".
+
+    #[local] Definition consumers_auth' γ_consumers i : iProp Σ :=
+      ∃ ηs,
+      mono_list_auth γ_consumers (DfracOwn 1) ηs ∗
+      ⌜length ηs = i⌝.
+    #[local] Definition consumers_auth γ :=
+      consumers_auth' γ.(inf_mpmc_queue_2_name_consumers).
+    #[local] Instance : CustomIpatFormat "consumers_auth" :=
+      " ( %ηs{} &
+          Hauth{} &
+          %Hηs{}
+        )
+      ".
+    #[local] Definition consumers_at γ i own : iProp Σ :=
+      ∃ η,
+      mono_list_at γ.(inf_mpmc_queue_2_name_consumers) i η ∗
+      match own with
+      | Own =>
+          oneshot_pending η (DfracOwn 1) ()
+      | Discard =>
+          oneshot_shot η ()
+      end.
+    #[local] Instance : CustomIpatFormat "consumers_at" :=
+      " ( %η{} &
+          Hat{_{}} &
+          Hη{}
+        )
+      ".
+    #[local] Definition consumers_lb γ i : iProp Σ :=
+      ∃ ηs,
+      mono_list_lb γ.(inf_mpmc_queue_2_name_consumers) ηs ∗
+      ⌜length ηs = i⌝.
+    #[local] Instance : CustomIpatFormat "consumers_lb" :=
+      " ( %ηs{} &
+          Hlb{} &
+          %Hηs{}
+        )
+      ".
+
+    #[local] Definition winner γ i : iProp Σ :=
+      ∃ id prophs,
+      wise_prophets_full global_prophet γ.(inf_mpmc_queue_2_name_prophet_name) i prophs ∗
+      ⌜head prophs = Some id⌝ ∗
+      identifier_model' id.
+    #[local] Instance : CustomIpatFormat "winner" :=
+      " ( %id{} &
+          %prophs{} &
+          Hprophet_full{_{}} &
+          %Hprophs{} &
+          Hid{}
+        )
+      ".
+
+    #[local] Definition consumer_au γ Ψ : iProp Σ :=
+      AU <{
+        ∃∃ vs,
+        model₁ γ vs
+      }> @ ⊤ ∖ ↑γ.(inf_mpmc_queue_2_name_inv), ∅ <{
+        ∀∀ v vs',
+        ⌜vs = v :: vs'⌝ ∗
+        model₁ γ vs'
+      , COMM
+        Ψ v
+      }>.
+
+    #[local] Definition inv_lstate_left γ back i lstate : iProp Σ :=
+      match lstate with
+      | ProducerProducer =>
+          ∃ v,
+          history_at γ i (Some v) ∗
+          winner γ i
+      | ProducerConsumer =>
+          history_at γ i None
+      | ConsumerProducer η =>
+          ∃ Ψ v,
+          consumers_lb γ (S i) ∗
+          saved_pred η Ψ ∗
+          history_at γ i (Some v) ∗
+          ( Ψ v
+          ∨ consumers_at γ i Discard
+          )
+      | ConsumerConsumer =>
+          consumers_lb γ (S i)
+      | _ =>
+          False
+      end.
+    #[local] Instance : CustomIpatFormat "inv_lstate_left_producer" :=
+      " ( %v &
+          #Hhistory_at &
+          Hwinner
+        )
+      ".
+    #[local] Instance : CustomIpatFormat "inv_lstate_left_consumer" :=
+      " ( %Ψ &
+          %v_ &
+          #Hconsumers_lb &
+          #Hη_ &
+          #Hhistory_at_ &
+          HΨ
+        )
+      ".
+
+    #[local] Definition inv_lstate_right γ i lstate : iProp Σ :=
+      match lstate with
+      | ConsumerProducer η =>
+          ∃ Ψ,
+          saved_pred η Ψ ∗
+          consumer_au γ Ψ
+      | ConsumerConsumer =>
+          winner γ i
+      | _ =>
+          False
+      end.
+    #[local] Instance : CustomIpatFormat "inv_lstate_right" :=
+      " ( %Ψ &
+          #Hη &
+          Hconsumer_au
+        )
+      ".
+
+    #[local] Definition inv_slot γ i slot past : iProp Σ :=
+      match slot with
+      | Nothing =>
+          ⌜past = []⌝
+      | Something v =>
+          history_at γ i (Some v) ∗
+          producers_at γ i Discard ∗
+          lstates_lb γ i Producer
+      | Anything =>
+          consumers_at γ i Discard ∗
+          ( lstates_lb γ i Consumer
+          ∨ producers_at γ i Discard
+          )
+      end.
+    #[local] Instance : CustomIpatFormat "inv_slot_nothing" :=
+      "%Hpast".
+    #[local] Instance : CustomIpatFormat "inv_slot_something" :=
+      " ( #Hhistory_at{_{suff}} &
+          #Hproducers_at{_{suff}} &
+          #Hlstates_lb_producer
+        )
+      ".
+    #[local] Instance : CustomIpatFormat "inv_slot_anything" :=
+      " ( #Hconsumers_at{_{suff}} &
+          { _{suff}
+          ; [ #Hlstates_lb_consumer
+            | #Hproducers_at_
+            ]
+          }
+        )
+      ".
+
+    #[local] Definition inv_inner t γ : iProp Σ :=
+      ∃ front back hist slots vs lstates pasts prophss,
+      t.[front] ↦ #front ∗
+      t.[back] ↦ #back ∗
+      inf_array_model γ.(inf_mpmc_queue_2_name_data) slots ∗
+      model₂ γ vs ∗
+      ⌜vs = oflatten (drop front hist)⌝ ∗
+      history_auth γ hist ∗
+      ⌜length hist = back⌝ ∗
+      lstates_auth γ lstates ∗
+      ⌜length lstates = front `max` back⌝ ∗
+      wise_prophets_model global_prophet γ.(inf_mpmc_queue_2_name_prophet) γ.(inf_mpmc_queue_2_name_prophet_name) pasts prophss ∗
+      producers_auth γ back ∗
+      consumers_auth γ front ∗
+      ( [∗ list] i ↦ lstate ∈ take back lstates,
+        inv_lstate_left γ back i lstate
+      ) ∗
+      ( [∗ list] k ↦ lstate ∈ drop back lstates,
+        inv_lstate_right γ (back + k) lstate
+      ) ∗
+      ( ∀ i,
+        inv_slot γ i (slots i) (pasts i)
+      ).
+    #[local] Instance : CustomIpatFormat "inv_inner" :=
+      " ( %front{} &
+          %back{} &
+          %hist{} &
+          %slots{} &
+          %vs{} &
+          %lstates{} &
+          %pasts{} &
+          %prophss{} &
+          Ht_front &
+          Ht_back &
+          >Hdata_model &
+          Hmodel₂ &
+          >%Hvs{} &
+          Hhistory_auth &
+          >%Hhist{} &
+          Hlstates_auth &
+          >%Hlstates{} &
+          >Hprophet_model &
+          Hproducers_auth &
+          Hconsumers_auth &
+          Hlstates_left &
+          Hlstates_right &
+          Hslots
+        )
+      ".
+    Definition inf_mpmc_queue_2_inv t γ ι : iProp Σ :=
+      ⌜ι = γ.(inf_mpmc_queue_2_name_inv)⌝ ∗
+      t.[data] ↦□ γ.(inf_mpmc_queue_2_name_data) ∗
+      t.[proph] ↦□ #γ.(inf_mpmc_queue_2_name_prophet) ∗
+      inf_array_inv γ.(inf_mpmc_queue_2_name_data) ∗
+      inv γ.(inf_mpmc_queue_2_name_inv) (inv_inner t γ).
+    #[local] Instance : CustomIpatFormat "inv" :=
+      " ( -> &
+          #Ht_data &
+          #Ht_proph &
+          #Hdata_inv &
+          #Hinv
+        )
+      ".
+
+    Definition inf_mpmc_queue_2_model :=
+      model₁.
+    #[local] Instance : CustomIpatFormat "model" :=
+      " Hmodel₁{_{}}
+      ".
+
+    #[global] Instance inf_mpmc_queue_2_model_timeless γ vs :
+      Timeless (inf_mpmc_queue_2_model γ vs).
+    Proof.
+      apply _.
+    Qed.
+
+    #[local] Instance lstates_at_persistent γ i lstate :
+      Persistent (lstates_at γ i lstate).
+    Proof.
+      apply _.
+    Qed.
+    #[local] Instance lstates_lb_persistent γ i lstate :
+      Persistent (lstates_lb γ i lstate).
+    Proof.
+      apply _.
+    Qed.
+    #[local] Instance producers_at_persistent γ i :
+      Persistent (producers_at γ i Discard).
+    Proof.
+      apply _.
+    Qed.
+    #[local] Instance consumers_at_persistent γ i :
+      Persistent (consumers_at γ i Discard).
+    Proof.
+      apply _.
+    Qed.
+    #[local] Instance consumers_lb_persistent γ i :
+      Persistent (consumers_lb γ i).
+    Proof.
+      apply _.
+    Qed.
+    #[local] Instance inv_slot_persistent γ i slot past :
+      Persistent (inv_slot γ i slot past).
+    Proof.
+      destruct slot; apply _.
+    Qed.
+    #[global] Instance inf_mpmc_queue_2_inv_persistent t γ ι :
+      Persistent (inf_mpmc_queue_2_inv t γ ι).
+    Proof.
+      apply _.
+    Qed.
+
+    #[local] Lemma model_alloc :
+      ⊢ |==>
+        ∃ γ_model,
+        model₁' γ_model [] ∗
+        model₂' γ_model [].
+    Proof.
+      apply twins_alloc'.
+    Qed.
+    #[local] Lemma model₁_exclusive γ vs1 vs2 :
+      model₁ γ vs1 -∗
+      model₁ γ vs2 -∗
+      False.
+    Proof.
+      apply twins_twin1_exclusive.
+    Qed.
+    #[local] Lemma model_agree γ vs1 vs2 :
+      model₁ γ vs1 -∗
+      model₂ γ vs2 -∗
+      ⌜vs1 = vs2⌝.
+    Proof.
+      apply: twins_agree_L.
+    Qed.
+    #[local] Lemma model_update {γ vs1 vs2} vs :
+      model₁ γ vs1 -∗
+      model₂ γ vs2 ==∗
+        model₁ γ vs ∗
+        model₂ γ vs.
+    Proof.
+      apply twins_update.
+    Qed.
+
+    #[local] Lemma history_alloc :
+      ⊢ |==>
+        ∃ γ_history,
+        history_auth' γ_history [].
+    Proof.
+      apply mono_list_alloc.
+    Qed.
+    #[local] Lemma history_at_lookup γ hist i o :
+      history_auth γ hist -∗
+      history_at γ i o -∗
+      ⌜hist !! i = Some o⌝.
+    Proof.
+      apply mono_list_at_valid.
+    Qed.
+    #[local] Lemma history_at_agree γ i o1 o2 :
+      history_at γ i o1 -∗
+      history_at γ i o2 -∗
+      ⌜o1 = o2⌝.
+    Proof.
+      iIntros "Hat1 Hat2".
+      iDestruct (mono_list_at_agree with "Hat1 Hat2") as %[= <-]. done.
+    Qed.
+    #[local] Lemma history_at_get {γ hist} i o :
+      hist !! i = Some o →
+      history_auth γ hist ⊢
+      history_at γ i o.
+    Proof.
+      apply mono_list_at_get.
+    Qed.
+    #[local] Lemma history_update {γ hist} o :
+      history_auth γ hist ⊢ |==>
+        history_auth γ (hist ++ [o]) ∗
+        history_at γ (length hist) o.
+    Proof.
+      iIntros "Hhistory_auth".
+      iMod (mono_list_update_snoc o with "Hhistory_auth") as "Hhistory_auth".
+      iDestruct (mono_list_at_get with "Hhistory_auth") as "#Hhistory_at".
+      { rewrite list_lookup_middle //. }
+      iSteps.
+    Qed.
+
+    #[local] Lemma lstates_alloc :
+      ⊢ |==>
+        ∃ γ_lstates,
+        lstates_auth' γ_lstates [].
+    Proof.
+      iMod (mono_list_alloc []) as "(%γ_lstates & $)".
+      iSteps.
+    Qed.
+    #[local] Lemma lstates_at_lookup γ lstates i lstate :
+      lstates_auth γ lstates -∗
+      lstates_at γ i lstate -∗
+      ⌜lstates !! i = Some lstate⌝.
+    Proof.
+      iIntros "(:lstates_auth) (:lstates_at)".
+      iDestruct (mono_list_at_valid with "Hauth Hat") as %Hηs_lookup.
+      iDestruct (big_sepL2_lookup_l with "Hηs") as "(%lstate_ & %Hlstates_lookup & Hη_auth_)"; first done.
+      iDestruct (auth_mono_auth_agree_L with "Hη_auth Hη_auth_") as %<-.
+      iSteps.
+    Qed.
+    #[local] Lemma lstates_lb_get {γ lstates} i lstate :
+      lstates !! i = Some lstate →
+      lstates_auth γ lstates -∗
+      lstates_lb γ i (lstate_winner lstate).
+    Proof.
+      iIntros "%Hlstates_lookup (:lstates_auth)".
+      iDestruct (big_sepL2_lookup_r with "Hηs") as "(%η & %Hηs_lookup & Hη_auth)"; first done.
+      iDestruct (auth_mono_lb_get with "Hη_auth") as "Hη_lb".
+      iDestruct (auth_mono_lb_mono with "Hη_lb") as "Hη_lb".
+      { apply lstate_winner_lb. }
+      iDestruct (mono_list_at_get with "Hauth") as "#Hat"; first done.
+      iSteps.
+    Qed.
+    #[local] Lemma lstates_lb_agree γ i lstate1 lstate2 :
+      lstates_lb γ i lstate1 -∗
+      lstates_lb γ i lstate2 -∗
+      ⌜lstate_winner lstate1 = lstate_winner lstate2⌝.
+    Proof.
+      iIntros "(:lstates_lb =1) (:lstates_lb =2)".
+      iDestruct (mono_list_at_agree with "Hat_1 Hat_2") as %<-.
+      iDestruct (auth_mono_lb_agree with "Hη_lb_1 Hη_lb_2") as %(lstate & ->%lsteps_winner & ->%lsteps_winner).
+      iSteps.
+    Qed.
+    #[local] Lemma lstates_update {γ lstates} lstate :
+      lstates_auth γ lstates ⊢ |==>
+        lstates_auth γ (lstates ++ [lstate]) ∗
+        lstates_lb γ (length lstates) (lstate_winner lstate) ∗
+        lstates_at γ (length lstates) lstate.
+    Proof.
+      iIntros "(:lstates_auth)".
+      iMod (auth_mono_alloc _ lstate) as "(%η & Hη_auth)".
+      iMod (auth_mono_auth_persist with "Hη_auth") as "#Hη_auth".
+      iMod (mono_list_update_snoc η with "Hauth") as "Hauth".
+      iDestruct (mono_list_at_get with "Hauth") as "#Hat".
+      { apply list_lookup_middle. done. }
+      iDestruct (auth_mono_lb_get with "Hη_auth") as "#Hη_lb".
+      iDestruct (auth_mono_lb_mono _ (lstate_winner lstate) with "Hη_lb") as "#Hη_lb_winner".
+      { destruct lstate; eauto using rtc, lstep. }
+      iDestruct (big_sepL2_length with "Hηs") as %->.
+      iDestruct (big_sepL2_snoc_2 with "Hηs Hη_auth") as "Hηs".
+      iSteps.
+    Qed.
+    Opaque lstates_auth'.
+    Opaque lstates_at.
+    Opaque lstates_lb.
+
+    #[local] Lemma producers_alloc :
+      ⊢ |==>
+        ∃ γ_producers,
+        producers_auth' γ_producers 0.
+    Proof.
+      iMod (mono_list_alloc []) as "(%γ_producers & $)".
+      iSteps.
+    Qed.
+    #[local] Lemma producers_at_exclusive γ i own :
+      producers_at γ i Own -∗
+      producers_at γ i own -∗
+      False.
+    Proof.
+      iIntros "(:producers_at =1) (:producers_at =2)".
+      iDestruct (mono_list_at_agree with "Hat_1 Hat_2") as %<-.
+      destruct own.
+      - iApply (oneshot_pending_exclusive with "Hη1 Hη2").
+      - iApply (oneshot_pending_shot with "Hη1 Hη2").
+    Qed.
+    #[local] Lemma producers_at_discard γ i :
+      producers_at γ i Own ⊢ |==>
+      producers_at γ i Discard.
+    Proof.
+      iIntros "(:producers_at)".
+      iMod (oneshot_update_shot with "Hη") as "Hη".
+      iSteps.
+    Qed.
+    #[local] Lemma producers_update γ i :
+      producers_auth γ i ⊢ |==>
+        producers_auth γ (S i) ∗
+        producers_at γ i Own.
+    Proof.
+      iIntros "(:producers_auth)".
+      iMod oneshot_alloc as "(%η & Hη_pending)".
+      iMod (mono_list_update_snoc η with "Hauth") as "Hauth".
+      iDestruct (mono_list_at_get with "Hauth") as "#Hat".
+      { apply list_lookup_middle. done. }
+      iSteps. simpl_length/=. iSteps.
+    Qed.
+    Opaque producers_auth'.
+    Opaque producers_at.
+
+    #[local] Lemma consumers_alloc :
+      ⊢ |==>
+        ∃ γ_consumers,
+        consumers_auth' γ_consumers 0.
+    Proof.
+      iMod (mono_list_alloc []) as "(%γ_consumers & $)".
+      iSteps.
+    Qed.
+    #[local] Lemma consumers_at_exclusive γ i own :
+      consumers_at γ i Own -∗
+      consumers_at γ i own -∗
+      False.
+    Proof.
+      iIntros "(:consumers_at =1) (:consumers_at =2)".
+      iDestruct (mono_list_at_agree with "Hat_1 Hat_2") as %<-.
+      destruct own.
+      - iApply (oneshot_pending_exclusive with "Hη1 Hη2").
+      - iApply (oneshot_pending_shot with "Hη1 Hη2").
+    Qed.
+    #[local] Lemma consumers_at_discard γ i :
+      consumers_at γ i Own ⊢ |==>
+      consumers_at γ i Discard.
+    Proof.
+      iIntros "(:consumers_at)".
+      iMod (oneshot_update_shot with "Hη") as "Hη".
+      iSteps.
+    Qed.
+    #[local] Lemma consumers_lb_valid γ i j :
+      consumers_auth γ i -∗
+      consumers_lb γ j -∗
+      ⌜j ≤ i⌝.
+    Proof.
+      iIntros "(:consumers_auth =1) (:consumers_lb =2)".
+      iDestruct (mono_list_lb_valid with "Hauth1 Hlb2") as %?%prefix_length.
+      iSteps.
+    Qed.
+    #[local] Lemma consumers_lb_le {γ i1} i2 :
+      i2 ≤ i1 →
+      consumers_lb γ i1 ⊢
+      consumers_lb γ i2.
+    Proof.
+      iIntros "% (:consumers_lb)".
+      iDestruct (mono_list_lb_mono (take i2 ηs) with "Hlb") as "$".
+      { apply prefix_take. }
+      simpl_length. iSteps.
+    Qed.
+    #[local] Lemma consumers_lb_get γ i :
+      consumers_auth γ i ⊢
+      consumers_lb γ i.
+    Proof.
+      iIntros "(:consumers_auth)".
+      iDestruct (mono_list_lb_get with "Hauth") as "Hlb".
+      iSteps.
+    Qed.
+    #[local] Lemma consumers_lb_get' {γ i} i' :
+      i' ≤ i →
+      consumers_auth γ i ⊢
+      consumers_lb γ i'.
+    Proof.
+      iIntros "% Hauth".
+      iDestruct (consumers_lb_get with "Hauth") as "Hlb".
+      iDestruct (consumers_lb_le with "Hlb") as "Hlb"; first done.
+      iSteps.
+    Qed.
+    #[local] Lemma consumers_update γ i :
+      consumers_auth γ i ⊢ |==>
+        consumers_auth γ (S i) ∗
+        consumers_at γ i Own.
+    Proof.
+      iIntros "(:consumers_auth)".
+      iMod oneshot_alloc as "(%η & Hη_pending)".
+      iMod (mono_list_update_snoc η with "Hauth") as "Hauth".
+      iDestruct (mono_list_at_get with "Hauth") as "#Hat".
+      { apply list_lookup_middle. done. }
+      iSteps. simpl_length/=. iSteps.
+    Qed.
+    Opaque consumers_auth'.
+    Opaque consumers_at.
+    Opaque consumers_lb.
+
+    #[local] Lemma winner_exclusive γ i :
+      winner γ i -∗
+      winner γ i -∗
+      False.
+    Proof.
+      iIntros "(:winner =1) (:winner =2)".
+      iDestruct (wise_prophets_full_agree with "Hprophet_full_1 Hprophet_full_2") as %->. simplify.
+      iApply (identifier_model_exclusive with "Hid1 Hid2").
+    Qed.
+
+    #[local] Lemma inv_slot_not_nothing_past {γ i slot past1} past2 :
+      slot ≠ Nothing →
+      inv_slot γ i slot past1 ⊣⊢
+      inv_slot γ i slot past2.
+    Proof.
+      destruct slot; iSteps.
+    Qed.
+
+    Lemma inf_mpmc_queue_2_model_exclusive γ vs1 vs2 :
+      inf_mpmc_queue_2_model γ vs1 -∗
+      inf_mpmc_queue_2_model γ vs2 -∗
+      False.
+    Proof.
+      iIntros "(:model =1) (:model =2)".
+      iApply (model₁_exclusive with "Hmodel₁_1 Hmodel₁_2").
+    Qed.
+
+    Lemma inf_mpmc_queue_2_create_spec ι :
+      {{{
+        True
+      }}}
+        inf_mpmc_queue_2_create ()
+      {{{ t γ,
+        RET #t;
+        meta_token t ⊤ ∗
+        inf_mpmc_queue_2_inv t γ ι ∗
+        inf_mpmc_queue_2_model γ []
+      }}}.
+    Proof.
+      iIntros "%Φ _ HΦ".
+
+      wp_rec.
+      wp_apply (wise_prophets_wp_proph global_prophet with "[//]") as "%pid %γ_prophet %prophss Hprophet_model".
+      wp_apply (inf_array_create_spec with "[//]") as (data) "(#Hdata_inv & Hdata_model)".
+      wp_block t as "Hmeta" "(Ht_data & Ht_front & Ht_back & Ht_proph & _)".
+      iMod (pointsto_persist with "Ht_data") as "#Ht_data".
+      iMod (pointsto_persist with "Ht_proph") as "#Ht_proph".
+
+      iMod model_alloc as "(%γ_model & Hmodel₁ & Hmodel₂)".
+      iMod history_alloc as "(%γ_history & Hhistory_auth)".
+      iMod lstates_alloc as "(%γ_lstates & Hlstates_auth)".
+      iMod producers_alloc as "(%γ_producers & Hproducers_auth)".
+      iMod consumers_alloc as "(%γ_consumers & Hconsumers_auth)".
+
+      pose γ := {|
+        inf_mpmc_queue_2_name_data := data ;
+        inf_mpmc_queue_2_name_inv := ι ;
+        inf_mpmc_queue_2_name_prophet := pid ;
+        inf_mpmc_queue_2_name_prophet_name := γ_prophet ;
+        inf_mpmc_queue_2_name_model := γ_model ;
+        inf_mpmc_queue_2_name_history := γ_history ;
+        inf_mpmc_queue_2_name_lstates := γ_lstates ;
+        inf_mpmc_queue_2_name_producers := γ_producers ;
+        inf_mpmc_queue_2_name_consumers := γ_consumers ;
+      |}.
+
+      iApply ("HΦ" $! t γ).
+      iFrameSteps. iExists (λ _, Nothing). iSteps. iExists []. iSteps.
+    Qed.
+
+    Lemma inf_mpmc_queue_2_size_spec t γ ι :
+      <<<
+        inf_mpmc_queue_2_inv t γ ι
+      | ∀∀ vs,
+        inf_mpmc_queue_2_model γ vs
+      >>>
+        inf_mpmc_queue_2_size #t @ ↑ι
+      <<<
+        inf_mpmc_queue_2_model γ vs
+      | sz,
+        RET #sz;
+        ⌜length vs ≤ sz⌝
+      >>>.
+    Proof.
+      iIntros "%Φ (:inv) HΦ".
+
+      iLöb as "HLöb".
+
+      wp_rec.
+
+      wp_bind (_.{front})%E.
+      iInv "Hinv" as "(:inv_inner =1)".
+      wp_load.
+      iDestruct (consumers_lb_get with "Hconsumers_auth") as "#Hconsumers_lb1".
+      iSplitR "HΦ". { iFrameSteps. }
+      iIntros "!> {%}".
+
+      wp_smart_apply (typed_prophet1_wp_proph local_prophet with "[//]") as (pid proph) "Hproph".
+      wp_pures.
+
+      wp_bind (_.{back})%E.
+      iInv "Hinv" as "(:inv_inner =2)".
+      wp_load.
+      destruct_decide (proph = front1) as -> | Hproph.
+
+      - destruct_decide (front2 = front1) as -> | ?.
+
+        + iMod "HΦ" as "(%vs & (:model) & _ & HΦ)".
+          iDestruct (model_agree with "Hmodel₁ Hmodel₂") as %->.
+          iMod ("HΦ" with "Hmodel₁") as "HΦ".
+
+          iSplitR "Hproph HΦ". { iFrameSteps. }
+          iModIntro. clear- Hvs2 Hhist2.
+
+          wp_pures.
+
+          wp_bind (_.{front})%E.
+          iInv "Hinv" as "(:inv_inner =3)".
+          wp_load.
+          iSplitR "Hproph HΦ". { iFrameSteps. }
+          iModIntro. clear -Hvs2 Hhist2.
+
+          wp_smart_apply (typed_prophet1_wp_resolve with "Hproph"); [done.. |].
+          iSteps. iPureIntro.
+          rewrite Hvs2. simpl_length. lia.
+
+        + iDestruct (consumers_lb_valid with "Hconsumers_auth Hconsumers_lb1") as %?.
+          iDestruct (consumers_lb_get with "Hconsumers_auth") as "#Hconsumers_lb2".
+          iSplitR "Hproph HΦ". { iFrameSteps. }
+          iModIntro.
+
+          wp_pures.
+
+          wp_bind (_.{front})%E.
+          iInv "Hinv" as "(:inv_inner =3)".
+          wp_load.
+          iDestruct (consumers_lb_valid with "Hconsumers_auth Hconsumers_lb2") as %?.
+          iSplitR "Hproph HΦ". { iFrameSteps. }
+          iModIntro.
+
+          wp_smart_apply (typed_prophet1_wp_resolve with "Hproph"); [done.. |].
+          iSteps.
+
+      - iSplitR "Hproph HΦ". { iFrameSteps. }
+        iModIntro. clear- Hproph.
+
+        wp_pures.
+
+        wp_bind (_.{front})%E.
+        iInv "Hinv" as "(:inv_inner =3)".
+        wp_load.
+        iSplitR "Hproph HΦ". { iFrameSteps. }
+        iModIntro. clear- Hproph.
+
+        wp_smart_apply (typed_prophet1_wp_resolve with "Hproph"); [done.. |].
+        iSteps.
+    Qed.
+
+    Lemma inf_mpmc_queue_2_is_empty_spec t γ ι :
+      <<<
+        inf_mpmc_queue_2_inv t γ ι
+      | ∀∀ vs,
+        inf_mpmc_queue_2_model γ vs
+      >>>
+        inf_mpmc_queue_2_is_empty #t @ ↑ι
+      <<<
+        inf_mpmc_queue_2_model γ vs
+      | b,
+        RET #b;
+        ⌜if b then vs = [] else True⌝
+      >>>.
+    Proof.
+      iIntros "%Φ #Hinv HΦ".
+
+      wp_rec.
+
+      awp_apply (inf_mpmc_queue_2_size_spec with "Hinv").
+      iApply (aacc_aupd_commit with "HΦ"); first done. iIntros "%vs Hmodel".
+      iAaccIntro with "Hmodel"; iSteps. iPureIntro.
+      case_bool_decide as Hlength; last done.
+      apply nil_length_inv. lia.
+    Qed.
+
+    Lemma inf_mpmc_queue_2_push_spec t γ ι v :
+      <<<
+        inf_mpmc_queue_2_inv t γ ι
+      | ∀∀ vs,
+        inf_mpmc_queue_2_model γ vs
+      >>>
+        inf_mpmc_queue_2_push #t v @ ↑ι
+      <<<
+        inf_mpmc_queue_2_model γ (vs ++ [v])
+      | RET ();
+        True
+      >>>.
+    Proof.
+      iIntros "%Φ (:inv) HΦ".
+
+      iLöb as "HLöb".
+
+      wp_rec.
+      wp_smart_apply (wp_id with "[//]") as (id) "Hid".
+      wp_pures.
+
+      wp_bind (FAA _ _).
+      iInv "Hinv" as "(:inv_inner =1)".
+      wp_faa.
+      iMod (producers_update with "Hproducers_auth") as "(Hproducers_auth & Hproducers_at)".
+      iDestruct (wise_prophets_full_get' _ back1 with "Hprophet_model") as "(%prophs & #Hprophet_full)".
+      destruct_decide (front1 ≤ back1) as Hfirst | Hlast.
+
+      - rewrite Nat.max_r // in Hlstates1.
+        rewrite firstn_all2; first lia.
+
+        destruct_decide (head prophs = Some id) as Hwinner | Hloser.
+
+        + iMod (history_update (Some v) with "Hhistory_auth") as "(Hhistory_auth & #Hhistory_at)". rewrite Hhist1.
+          iMod (lstates_update ProducerProducer with "Hlstates_auth") as "(Hlstates_auth & #Hlstates_lb & _)". rewrite Hlstates1.
+          iDestruct (big_sepL_snoc_2 ProducerProducer with "Hlstates_left [Hid]") as "Hlstates_left".
+          { rewrite Hlstates1. iSteps. }
+
+          iMod "HΦ" as "(%vs & (:model) & _ & HΦ)".
+          iDestruct (model_agree with "Hmodel₁ Hmodel₂") as %<-.
+          iMod (model_update (vs ++ [v]) with "Hmodel₁ Hmodel₂") as "(Hmodel₁ & Hmodel₂)".
+          iMod ("HΦ" with "Hmodel₁ [//]") as "HΦ".
+
+          iSplitR "Hproducers_at HΦ".
+          { iFrame.
+            rewrite firstn_all2. { simpl_length/=. lia. }
+            rewrite (skipn_all2 (n := S back1)).
+            { simpl_length/=. lia. }
+            iFrameSteps; iPureIntro.
+            - rewrite drop_app_le; first lia.
+              rewrite oflatten_snoc_Some Hvs1 //.
+            - simpl_length/=. lia.
+            - simpl_length/=. lia.
+          }
+          iModIntro. clear- Hwinner.
+
+          do 2 wp_load.
+
+          wp_apply (inf_array_cas_resolve_spec with "Hdata_inv"); first lia.
+          iMod (inv_acc with "Hinv") as "((:inv_inner =2) & Hclose1)"; first done.
+          iStep. iIntros "%e %b % % %Hslots2 Hdata_model".
+          rewrite Nat2Z.id in Hslots2 |- *.
+          wp_apply (wise_prophets_wp_resolve' with "Hprophet_model"); [done.. |].
+          wp_pures.
+          iIntros "!> %prophs2 %Hprophss2 Hprophet_model".
+          destruct b; last first.
+          { iDestruct ("Hslots" $! back1) as "Hslot".
+            destruct (slots2 back1).
+            - exfalso. done.
+            - iDestruct "Hslot" as "(:inv_slot_anything)".
+              + iDestruct (lstates_lb_agree with "Hlstates_lb Hlstates_lb_consumer") as %[=].
+              + iDestruct (producers_at_exclusive with "Hproducers_at Hproducers_at_") as %[].
+            - iDestruct "Hslot" as "(:inv_slot_something suff=)".
+              iDestruct (producers_at_exclusive with "Hproducers_at Hproducers_at_") as %[].
+          }
+          iMod (producers_at_discard with "Hproducers_at") as "#Hproducers_at".
+          iMod ("Hclose1" with "[- HΦ]") as "_".
+          { rewrite -(fn_compose_insert _ _ _ (Something v)).
+            iFrameSteps.
+            rewrite function.fn_lookup_insert. case_decide.
+            - subst. iSteps.
+            - rewrite fn_lookup_alter_ne //.
+          }
+          iSteps.
+
+        + iMod (history_update None with "Hhistory_auth") as "(Hhistory_auth & #Hhistory_at)". rewrite Hhist1.
+          iMod (lstates_update ProducerConsumer with "Hlstates_auth") as "(Hlstates_auth & Hlstates_lb & _)".
+          iDestruct (big_sepL_snoc_2 ProducerConsumer with "Hlstates_left []") as "Hlstates_left".
+          { rewrite Hlstates1 //. }
+          iSplitR "HΦ".
+          { iFrame.
+            rewrite firstn_all2. { simpl_length/=. lia. }
+            rewrite (skipn_all2 (n := S back1)).
+            { simpl_length/=. lia. }
+            iFrameSteps; iPureIntro.
+            - rewrite drop_app_le; first lia.
+              rewrite oflatten_snoc_None Hvs1 //.
+            - simpl_length/=. lia.
+            - simpl_length/=. lia.
+          }
+          iModIntro. clear- Hloser.
+
+          do 2 wp_load.
+
+          wp_apply (inf_array_cas_resolve_spec with "Hdata_inv"); first lia.
+          iMod (inv_acc with "Hinv") as "((:inv_inner =2) & Hclose1)"; first done.
+          iStep. iIntros "%e %b % % %Hslots2 Hdata_model".
+          rewrite Nat2Z.id in Hslots2 |- *.
+          wp_apply (wise_prophets_wp_resolve' with "Hprophet_model"); [done.. |].
+          wp_pures.
+          iIntros "!> %prophs2 %Hprophss2 Hprophet_model".
+          destruct b.
+          { iDestruct ("Hslots" $! back1) as "Hslot".
+            destruct (slots2 back1).
+            - iDestruct "Hslot" as "(:inv_slot_nothing)".
+              iDestruct (wise_prophets_full_valid with "Hprophet_model Hprophet_full") as %Hprophs.
+              exfalso.
+              rewrite fn_lookup_alter Hpast /= in Hprophs. naive_solver.
+            - exfalso. done.
+            - exfalso. done.
+          }
+          iMod ("Hclose1" with "[- HΦ]") as "_".
+          { iFrameSteps.
+            rewrite function.fn_lookup_alter. case_decide; last done.
+            subst. rewrite inv_slot_not_nothing_past //.
+            intros Heq. rewrite Heq // in Hslots2.
+          }
+          iSteps.
+
+      - rewrite drop_ge /= in Hvs1; first lia. subst vs1.
+        rewrite Nat.max_l in Hlstates1; first lia.
+        iDestruct (consumers_lb_get' (S back1) with "Hconsumers_auth") as "#Hconsumers_lb"; first lia.
+        destruct (lookup_lt_is_Some_2 lstates1 back1) as (lstate & Hlstates_lookup); first lia.
+        iDestruct (lstates_lb_get with "Hlstates_auth") as "#Hlstates_lb"; first done.
+        erewrite drop_S; last done.
+        iDestruct "Hlstates_right" as "(Hlstate & Hlstates_right)".
+
+        destruct lstate as [| | | | η |].
+        all: try iDestruct "Hlstate" as %[].
+
+        + iDestruct "Hlstate" as "(:inv_lstate_right)".
+
+          iMod "HΦ" as "(%vs & (:model) & _ & HΦ)".
+          iDestruct (model_agree with "Hmodel₁ Hmodel₂") as %->.
+          iMod (model_update [v] with "Hmodel₁ Hmodel₂") as "(Hmodel₁ & Hmodel₂)".
+          iMod ("HΦ" with "Hmodel₁ [//]") as "HΦ".
+
+          iMod "Hconsumer_au" as "(%vs & Hmodel₁ & _ & HΨ)".
+          iDestruct (model_agree with "Hmodel₁ Hmodel₂") as %->.
+          iMod (model_update [] with "Hmodel₁ Hmodel₂") as "(Hmodel₁ & Hmodel₂)".
+          iMod ("HΨ" with "[$Hmodel₁ //]") as "HΨ".
+
+          iMod (history_update (Some v) with "Hhistory_auth") as "(Hhistory_auth & #Hhistory_lb)". rewrite Hhist1.
+          iDestruct (big_sepL_snoc_2 (ConsumerProducer η) with "Hlstates_left [HΨ]") as "Hlstates_left".
+          { rewrite /= length_take Nat.min_l; first lia. iSteps. }
+          iSplitR "Hproducers_at HΦ".
+          { rewrite -take_S_r //.
+            setoid_rewrite Nat.add_succ_r.
+            iFrameSteps; iPureIntro.
+            - rewrite drop_ge //. { simpl_length/=. lia. }
+            - simpl_length/=. lia.
+          }
+          iIntros "!> {%}".
+
+          do 2 wp_load.
+
+          wp_apply (inf_array_cas_resolve_spec with "Hdata_inv"); first lia.
+          iMod (inv_acc with "Hinv") as "((:inv_inner =2) & Hclose1)"; first done.
+          iStep. iIntros "%e %b % % %Hslots2 Hdata_model".
+          rewrite Nat2Z.id in Hslots2 |- *.
+          wp_apply (wise_prophets_wp_resolve' with "Hprophet_model"); [done.. |].
+          wp_pures.
+          iIntros "!> %prophs2 %Hprophss2 Hprophet_model".
+          destruct b; last first.
+          { iDestruct ("Hslots" $! back1) as "Hslot".
+            destruct (slots2 back1).
+            - iDestruct "Hslot" as "(:inv_slot_nothing)".
+              iDestruct (wise_prophets_full_valid with "Hprophet_model Hprophet_full") as %Hprophs.
+              exfalso.
+              rewrite fn_lookup_alter Hpast /= in Hprophs. naive_solver.
+            - iDestruct "Hslot" as "(:inv_slot_anything)".
+              + iDestruct (lstates_lb_agree with "Hlstates_lb Hlstates_lb_consumer") as %[=].
+              + iDestruct (producers_at_exclusive with "Hproducers_at Hproducers_at_") as %[].
+            - iDestruct "Hslot" as "(:inv_slot_something suff=)".
+              iDestruct (producers_at_exclusive with "Hproducers_at Hproducers_at_") as %[].
+          }
+          iMod (producers_at_discard with "Hproducers_at") as "#Hproducers_at".
+          iMod ("Hclose1" with "[- HΦ]") as "_".
+          { rewrite -(fn_compose_insert _ _ _ (Something v)).
+            iFrameSteps.
+            rewrite function.fn_lookup_insert. case_decide.
+            - subst. iSteps.
+            - rewrite fn_lookup_alter_ne //.
+          }
+          iSteps.
+
+        + iAssert ⌜head prophs ≠ Some id⌝%I as %Hloser.
+          { iIntros (Hwinner).
+            iEval (rewrite /= Nat.add_0_r) in "Hlstate".
+            iDestruct (winner_exclusive with "Hlstate [Hid]") as %[]; first iSteps.
+          }
+
+          iMod (history_update None with "Hhistory_auth") as "(Hhistory_auth & _)".
+          iDestruct (big_sepL_snoc_2 ConsumerConsumer with "Hlstates_left []") as "Hlstates_left".
+          { rewrite /= length_take Nat.min_l; first lia. iSteps. }
+          iSplitR "HΦ".
+          { rewrite -take_S_r //.
+            setoid_rewrite Nat.add_succ_r.
+            iFrameSteps; iPureIntro.
+            - rewrite drop_ge //. { simpl_length/=. lia. }
+            - simpl_length/=. lia.
+          }
+          iModIntro. clear- Hloser.
+
+          do 2 wp_load.
+
+          wp_apply (inf_array_cas_resolve_spec with "Hdata_inv"); first lia.
+          iMod (inv_acc with "Hinv") as "((:inv_inner =2) & Hclose1)"; first done.
+          iStep. iIntros "%e %b % % %Hslots2 Hdata_model".
+          rewrite Nat2Z.id in Hslots2 |- *.
+          wp_apply (wise_prophets_wp_resolve' with "Hprophet_model"); [done.. |].
+          wp_pures.
+          iIntros "!> %prophs2 %Hprophss2 Hprophet_model".
+          destruct b.
+          { iDestruct ("Hslots" $! back1) as "Hslot".
+            destruct (slots2 back1).
+            - iDestruct "Hslot" as "(:inv_slot_nothing)".
+              iDestruct (wise_prophets_full_valid with "Hprophet_model Hprophet_full") as %Hprophs.
+              exfalso.
+              rewrite fn_lookup_alter Hpast /= in Hprophs. naive_solver.
+            - exfalso. done.
+            - exfalso. done.
+          }
+          iMod ("Hclose1" with "[- HΦ]") as "_".
+          { iFrameSteps.
+            rewrite function.fn_lookup_alter. case_decide; last done.
+            subst. rewrite inv_slot_not_nothing_past //.
+            intros Heq. rewrite Heq // in Hslots2.
+          }
+          iSteps.
+    Qed.
+
+    Lemma inf_mpmc_queue_2_pop_spec t γ ι :
+      <<<
+        inf_mpmc_queue_2_inv t γ ι
+      | ∀∀ vs,
+        inf_mpmc_queue_2_model γ vs
+      >>>
+        inf_mpmc_queue_2_pop #t @ ↑ι
+      <<<
+        ∃∃ v vs',
+        ⌜vs = v :: vs'⌝ ∗
+        inf_mpmc_queue_2_model γ vs'
+      | RET v;
+        True
+      >>>.
+    Proof.
+      iIntros "%Φ (:inv) HΦ".
+
+      iLöb as "HLöb".
+
+      wp_rec.
+      wp_smart_apply (wp_id with "[//]") as (id) "Hid".
+      wp_pures.
+
+      wp_bind (FAA _ _).
+      iInv "Hinv" as "(:inv_inner =1)".
+      wp_faa.
+      iDestruct (wise_prophets_full_get' _ front1 with "Hprophet_model") as "(%prophs & #Hprophet_full)".
+      destruct_decide (back1 ≤ front1) as Hfirst | Hlast.
+
+      - rewrite drop_ge /= in Hvs1; first lia. subst vs1.
+        rewrite Nat.max_l // in Hlstates1.
+
+        iMod (consumers_update with "Hconsumers_auth") as "(Hconsumers_auth & Hconsumers_at)".
+
+        destruct_decide (head prophs = Some id) as Hwinner | Hloser.
+
+        + iMod (lstates_update ConsumerConsumer with "Hlstates_auth") as "(Hlstates_auth & #Hlstates_lb & _)". rewrite Hlstates1.
+          iDestruct (big_sepL_snoc_2 ConsumerConsumer with "Hlstates_right [Hid]") as "Hlstates_right".
+          { rewrite length_drop Hlstates1 -Nat.le_add_sub; first lia.
+            iSteps.
+          }
+
+          iSplitR "Hconsumers_at HΦ".
+          { iFrame.
+            rewrite (drop_ge hist1); first lia.
+            rewrite take_app_le; first lia.
+            rewrite drop_app_le; first lia.
+            iFrameSteps. iPureIntro.
+            simpl_length/=. lia.
+          }
+          iModIntro. clear- Hwinner.
+
+          do 2 wp_load.
+
+          wp_apply (inf_array_xchg_resolve_spec with "Hdata_inv"); first lia.
+          iMod (inv_acc with "Hinv") as "((:inv_inner =2) & Hclose1)"; first done.
+          iStep. iIntros "%e % % Hdata_model".
+          rewrite Nat2Z.id.
+          wp_apply (wise_prophets_wp_resolve' with "Hprophet_model"); [done.. |].
+          wp_pures.
+          iIntros "!> %prophs2 %Hprophss2 Hprophet_model".
+          iDestruct (bi.forall_elim front1 with "Hslots") as "#-#Hslot".
+          destruct (slots2 front1); first last.
+          { iDestruct "Hslot" as "(:inv_slot_something)".
+            iDestruct (lstates_lb_agree with "Hlstates_lb Hlstates_lb_producer") as %[=].
+          } {
+            iDestruct "Hslot" as "(:inv_slot_anything suff=)".
+            iDestruct (consumers_at_exclusive with "Hconsumers_at Hconsumers_at_") as %[].
+          }
+          iMod (consumers_at_discard with "Hconsumers_at") as "#Hconsumers_at".
+          iMod ("Hclose1" with "[- HΦ]") as "_".
+          { rewrite -(fn_compose_insert _ _ _ Anything).
+            iFrameSteps.
+            rewrite function.fn_lookup_insert. case_decide.
+            - subst. iSteps.
+            - rewrite fn_lookup_alter_ne //.
+          }
+          iSteps.
+
+        + iMod (saved_pred_alloc Φ) as "(%η & #Hη)".
+          iMod (lstates_update (ConsumerProducer η) with "Hlstates_auth") as "(Hlstates_auth & _ & #Hlstates_at)". rewrite Hlstates1.
+          iDestruct (big_sepL_snoc_2 (ConsumerProducer η) with "Hlstates_right [HΦ]") as "Hlstates_right".
+          { iSteps.
+            rewrite /consumer_au. iAuIntro.
+            iApply (aacc_aupd_commit with "HΦ"); first done. iIntros "%vs (:model)".
+            iAaccIntro with "Hmodel₁"; iSteps.
+          }
+
+          iSplitR "Hconsumers_at".
+          { iFrame.
+            rewrite (drop_ge hist1); first lia.
+            rewrite take_app_le; first lia.
+            rewrite drop_app_le; first lia.
+            iFrameSteps. iPureIntro.
+            simpl_length/=. lia.
+          }
+          iModIntro. clear- Hloser.
+
+          do 2 wp_load.
+
+          wp_apply (inf_array_xchg_resolve_spec with "Hdata_inv"); first lia.
+          iMod (inv_acc with "Hinv") as "((:inv_inner =2) & Hclose1)"; first done.
+          iStep. iIntros "%e % % Hdata_model".
+          rewrite Nat2Z.id.
+          wp_apply (wise_prophets_wp_resolve' with "Hprophet_model"); [done.. |].
+          wp_pures.
+          iIntros "!> %prophs2 %Hprophss2 Hprophet_model".
+          iDestruct (bi.forall_elim front1 with "Hslots") as "#-#Hslot".
+          destruct (slots2 front1) as [| | v].
+          { iDestruct "Hslot" as "(:inv_slot_nothing)".
+            iDestruct (wise_prophets_full_valid with "Hprophet_model Hprophet_full") as %Hprophs.
+            exfalso.
+            rewrite fn_lookup_alter Hpast /= in Hprophs. naive_solver.
+          } {
+            iDestruct "Hslot" as "(:inv_slot_anything suff=)".
+            iDestruct (consumers_at_exclusive with "Hconsumers_at Hconsumers_at_") as %[].
+          }
+          iDestruct "Hslot" as "(:inv_slot_something)".
+
+          iDestruct (lstates_at_lookup with "Hlstates_auth Hlstates_at") as %Hlstates2_lookup.
+          iDestruct (history_at_lookup with "Hhistory_auth Hhistory_at") as %?%lookup_lt_Some.
+          iDestruct (big_sepL_lookup_acc with "Hlstates_left") as "(Hlstate & Hlstates_left)".
+          { rewrite lookup_take_Some. naive_solver. }
+          iDestruct "Hlstate" as "(:inv_lstate_left_consumer suff=)".
+          iDestruct (history_at_agree with "Hhistory_at Hhistory_at_") as %[= <-].
+          iDestruct (saved_pred_agree v with "Hη Hη_") as "#Heq".
+          iDestruct "HΨ" as "[HΦ | Hconsumers_at_]"; last first.
+          { iDestruct (consumers_at_exclusive with "Hconsumers_at Hconsumers_at_") as %[]. }
+
+          iMod (consumers_at_discard with "Hconsumers_at") as "#Hconsumers_at".
+          iMod ("Hclose1" with "[- HΦ]") as "_".
+          { rewrite -(fn_compose_insert _ _ _ Anything).
+            iFrameSteps.
+            rewrite function.fn_lookup_insert. case_decide.
+            - subst. iSteps.
+            - rewrite fn_lookup_alter_ne //.
+          }
+          iIntros "!> {%}".
+
+          wp_pures.
+          iRewrite "Heq". iSteps.
+
+      - rewrite Nat.max_r in Hlstates1; first lia.
+        destruct (lookup_lt_is_Some_2 lstates1 front1) as (lstate & Hlstates_lookup); first lia.
+        iDestruct (big_sepL_lookup_acc with "Hlstates_left") as "(Hlstate & Hlstates_left)".
+        { rewrite lookup_take_Some. naive_solver lia. }
+        destruct lstate.
+        all: try iDestruct "Hlstate" as %[].
+        1,2: iMod (consumers_update with "Hconsumers_auth") as "(Hconsumers_auth & Hconsumers_at)".
+
+        + iDestruct "Hlstate" as "(:inv_lstate_left_producer)".
+          iDestruct (history_at_lookup with "Hhistory_auth Hhistory_at") as %Hhist1_lookup.
+          erewrite drop_S, oflatten_cons_Some in Hvs1; last done.
+
+          iAssert ⌜head prophs ≠ Some id⌝%I as %Hloser.
+          { iIntros (Hwinner).
+            iDestruct (winner_exclusive with "Hwinner [Hid]") as %[]; first iSteps.
+          }
+
+          iMod "HΦ" as "(%vs & (:model) & _ & HΦ)".
+          iDestruct (model_agree with "Hmodel₁ Hmodel₂") as %<-.
+          iMod (model_update with "Hmodel₁ Hmodel₂") as "(Hmodel₁ & Hmodel₂)".
+          iMod ("HΦ" with "[$Hmodel₁ //] [//]") as "HΦ".
+
+          iSplitR "Hconsumers_at HΦ". { iFrameSteps. }
+          iModIntro. clear- Hloser.
+
+          do 2 wp_load.
+
+          wp_apply (inf_array_xchg_resolve_spec with "Hdata_inv"); first lia.
+          iMod (inv_acc with "Hinv") as "((:inv_inner =2) & Hclose1)"; first done.
+          iStep. iIntros "%e % % Hdata_model".
+          rewrite Nat2Z.id.
+          wp_apply (wise_prophets_wp_resolve' with "Hprophet_model"); [done.. |].
+          wp_pures.
+          iIntros "!> %prophs2 %Hprophss2 Hprophet_model".
+          iDestruct (bi.forall_elim front1 with "Hslots") as "#-#Hslot".
+          destruct (slots2 front1) as [| | v_].
+          { iDestruct "Hslot" as "(:inv_slot_nothing)".
+            iDestruct (wise_prophets_full_valid with "Hprophet_model Hprophet_full") as %Hprophs.
+            exfalso.
+            rewrite fn_lookup_alter Hpast /= in Hprophs. naive_solver.
+          } {
+            iDestruct "Hslot" as "(:inv_slot_anything suff=)".
+            iDestruct (consumers_at_exclusive with "Hconsumers_at Hconsumers_at_") as %[].
+          }
+          iDestruct "Hslot" as "(:inv_slot_something suff=)".
+          iDestruct (history_at_agree with "Hhistory_at Hhistory_at_") as %[= <-].
+          iMod (consumers_at_discard with "Hconsumers_at") as "#Hconsumers_at".
+          iMod ("Hclose1" with "[- HΦ]") as "_".
+          { rewrite -(fn_compose_insert _ _ _ Anything).
+            iFrameSteps.
+            rewrite function.fn_lookup_insert. case_decide.
+            - subst. iSteps.
+            - rewrite fn_lookup_alter_ne //.
+          }
+          iSteps.
+
+        + iDestruct (history_at_lookup with "Hhistory_auth Hlstate") as %Hhist1_lookup.
+          erewrite drop_S, oflatten_cons_None in Hvs1; last done.
+          iDestruct (lstates_lb_get with "Hlstates_auth") as "#Hlstates_lb"; first done.
+
+          iSplitR "Hconsumers_at HΦ". { iFrameSteps. }
+          iIntros "!> {%}".
+
+          do 2 wp_load.
+
+          wp_apply (inf_array_xchg_resolve_spec with "Hdata_inv"); first lia.
+          iMod (inv_acc with "Hinv") as "((:inv_inner =2) & Hclose1)"; first done.
+          iStep. iIntros "%e % % Hdata_model".
+          rewrite Nat2Z.id.
+          wp_apply (wise_prophets_wp_resolve' with "Hprophet_model"); [done.. |].
+          wp_pures.
+          iIntros "!> %prophs2 %Hprophss2 Hprophet_model".
+          iDestruct (bi.forall_elim front1 with "Hslots") as "#-#Hslot".
+          destruct (slots2 front1) as [| | v]; first last.
+          { iDestruct "Hslot" as "(:inv_slot_something)".
+            iDestruct (lstates_lb_agree with "Hlstates_lb Hlstates_lb_producer") as %[=].
+          } {
+            iDestruct "Hslot" as "(:inv_slot_anything suff=)".
+            iDestruct (consumers_at_exclusive with "Hconsumers_at Hconsumers_at_") as %[].
+          }
+          iMod (consumers_at_discard with "Hconsumers_at") as "#Hconsumers_at".
+          iMod ("Hclose1" with "[- HΦ]") as "_".
+          { rewrite -(fn_compose_insert _ _ _ Anything).
+            iFrameSteps.
+            rewrite function.fn_lookup_insert. case_decide.
+            - subst. iSteps.
+            - rewrite fn_lookup_alter_ne //.
+          }
+          iSteps.
+
+        + iDestruct "Hlstate" as "(:inv_lstate_left_consumer)".
+          iDestruct (consumers_lb_valid with "Hconsumers_auth Hconsumers_lb") as %?. lia.
+
+        + iDestruct (consumers_lb_valid with "Hconsumers_auth Hlstate") as %?. lia.
+    Qed.
+  End inf_mpmc_queue_2_G.
+
+  #[global] Opaque inf_mpmc_queue_2_inv.
+  #[global] Opaque inf_mpmc_queue_2_model.
+End base.
+
+From zoo_saturn Require
+  inf_mpmc_queue_2__opaque.
+
 Section inf_mpmc_queue_2_G.
   Context `{inf_mpmc_queue_2_G : InfMpmcQueue2G Σ}.
 
-  Implicit Types Ψ : val → iProp Σ.
+  Implicit Types 𝑡 : location.
+  Implicit Types t : val.
 
-  Record metadata := {
-    metadata_data : val ;
-    metadata_inv : namespace ;
-    metadata_prophet : prophet_id ;
-    metadata_prophet_name : wise_prophets_name ;
-    metadata_model : gname ;
-    metadata_history : gname ;
-    metadata_lstates : gname ;
-    metadata_producers : gname ;
-    metadata_consumers : gname ;
-  }.
-  Implicit Type γ : metadata.
-
-  #[local] Instance metadata_eq_dec : EqDecision metadata :=
-    ltac:(solve_decision).
-  #[local] Instance metadata_countable :
-    Countable metadata.
-  Proof.
-    solve_countable.
-  Qed.
-
-  #[local] Definition model₁' γ_model vs :=
-    twins_twin1 γ_model (DfracOwn 1) vs.
-  #[local] Definition model₁ γ vs :=
-    model₁' γ.(metadata_model) vs.
-  #[local] Definition model₂' γ_model vs :=
-    twins_twin2 γ_model vs.
-  #[local] Definition model₂ γ vs :=
-    model₂' γ.(metadata_model) vs.
-
-  #[local] Definition history_auth' γ_history hist :=
-    mono_list_auth γ_history (DfracOwn 1) hist.
-  #[local] Definition history_auth γ :=
-    history_auth' γ.(metadata_history).
-  #[local] Definition history_at γ i o :=
-    mono_list_at γ.(metadata_history) i o.
-
-  #[local] Definition lstates_auth' γ_lstates lstates : iProp Σ :=
-    ∃ ηs,
-    mono_list_auth γ_lstates (DfracOwn 1) ηs ∗
-    [∗ list] η; lstate ∈ ηs; lstates,
-      auth_mono_auth _ η DfracDiscarded lstate.
-  #[local] Definition lstates_auth γ :=
-    lstates_auth' γ.(metadata_lstates).
-  #[local] Instance : CustomIpatFormat "lstates_auth" :=
-    " ( %ηs &
-        Hauth &
-        Hηs
-      )
-    ".
-  #[local] Definition lstates_at γ i lstate : iProp Σ :=
-    ∃ η,
-    mono_list_at γ.(metadata_lstates) i η ∗
-    auth_mono_auth _ η DfracDiscarded lstate.
-  #[local] Instance : CustomIpatFormat "lstates_at" :=
-    " ( %η{} &
-        #Hat{_{}} &
-        #Hη_auth{_{}}
-      )
-    ".
-  #[local] Definition lstates_lb γ i lstate : iProp Σ :=
-    ∃ η,
-    mono_list_at γ.(metadata_lstates) i η ∗
-    auth_mono_lb _ η lstate.
-  #[local] Instance : CustomIpatFormat "lstates_lb" :=
-    " ( %η{} &
-        #Hat{_{}} &
-        #Hη_lb{_{}}
-      )
-    ".
-
-  #[local] Definition producers_auth' γ_producers i : iProp Σ :=
-    ∃ ηs,
-    mono_list_auth γ_producers (DfracOwn 1) ηs ∗
-    ⌜length ηs = i⌝.
-  #[local] Definition producers_auth γ :=
-    producers_auth' γ.(metadata_producers).
-  #[local] Instance : CustomIpatFormat "producers_auth" :=
-    " ( %ηs &
-        Hauth &
-        %Hηs
-      )
-    ".
-  #[local] Definition producers_at γ i own : iProp Σ :=
-    ∃ η,
-    mono_list_at γ.(metadata_producers) i η ∗
-    match own with
-    | Own =>
-        oneshot_pending η (DfracOwn 1) ()
-    | Discard =>
-        oneshot_shot η ()
-    end.
-  #[local] Instance : CustomIpatFormat "producers_at" :=
-    " ( %η{} &
-        Hat{_{}} &
-        Hη{}
-      )
-    ".
-
-  #[local] Definition consumers_auth' γ_consumers i : iProp Σ :=
-    ∃ ηs,
-    mono_list_auth γ_consumers (DfracOwn 1) ηs ∗
-    ⌜length ηs = i⌝.
-  #[local] Definition consumers_auth γ :=
-    consumers_auth' γ.(metadata_consumers).
-  #[local] Instance : CustomIpatFormat "consumers_auth" :=
-    " ( %ηs{} &
-        Hauth{} &
-        %Hηs{}
-      )
-    ".
-  #[local] Definition consumers_at γ i own : iProp Σ :=
-    ∃ η,
-    mono_list_at γ.(metadata_consumers) i η ∗
-    match own with
-    | Own =>
-        oneshot_pending η (DfracOwn 1) ()
-    | Discard =>
-        oneshot_shot η ()
-    end.
-  #[local] Instance : CustomIpatFormat "consumers_at" :=
-    " ( %η{} &
-        Hat{_{}} &
-        Hη{}
-      )
-    ".
-  #[local] Definition consumers_lb γ i : iProp Σ :=
-    ∃ ηs,
-    mono_list_lb γ.(metadata_consumers) ηs ∗
-    ⌜length ηs = i⌝.
-  #[local] Instance : CustomIpatFormat "consumers_lb" :=
-    " ( %ηs{} &
-        Hlb{} &
-        %Hηs{}
-      )
-    ".
-
-  #[local] Definition winner γ i : iProp Σ :=
-    ∃ id prophs,
-    wise_prophets_full global_prophet γ.(metadata_prophet_name) i prophs ∗
-    ⌜head prophs = Some id⌝ ∗
-    identifier_model' id.
-  #[local] Instance : CustomIpatFormat "winner" :=
-    " ( %id{} &
-        %prophs{} &
-        Hprophet_full{_{}} &
-        %Hprophs{} &
-        Hid{}
-      )
-    ".
-
-  #[local] Definition consumer_au γ Ψ : iProp Σ :=
-    AU <{
-      ∃∃ vs,
-      model₁ γ vs
-    }> @ ⊤ ∖ ↑γ.(metadata_inv), ∅ <{
-      ∀∀ v vs',
-      ⌜vs = v :: vs'⌝ ∗
-      model₁ γ vs'
-    , COMM
-      Ψ v
-    }>.
-
-  #[local] Definition inv_lstate_left γ back i lstate : iProp Σ :=
-    match lstate with
-    | ProducerProducer =>
-        ∃ v,
-        history_at γ i (Some v) ∗
-        winner γ i
-    | ProducerConsumer =>
-        history_at γ i None
-    | ConsumerProducer η =>
-        ∃ Ψ v,
-        consumers_lb γ (S i) ∗
-        saved_pred η Ψ ∗
-        history_at γ i (Some v) ∗
-        ( Ψ v
-        ∨ consumers_at γ i Discard
-        )
-    | ConsumerConsumer =>
-        consumers_lb γ (S i)
-    | _ =>
-        False
-    end.
-  #[local] Instance : CustomIpatFormat "inv_lstate_left_producer" :=
-    " ( %v &
-        #Hhistory_at &
-        Hwinner
-      )
-    ".
-  #[local] Instance : CustomIpatFormat "inv_lstate_left_consumer" :=
-    " ( %Ψ &
-        %v_ &
-        #Hconsumers_lb &
-        #Hη_ &
-        #Hhistory_at_ &
-        HΨ
-      )
-    ".
-
-  #[local] Definition inv_lstate_right γ i lstate : iProp Σ :=
-    match lstate with
-    | ConsumerProducer η =>
-        ∃ Ψ,
-        saved_pred η Ψ ∗
-        consumer_au γ Ψ
-    | ConsumerConsumer =>
-        winner γ i
-    | _ =>
-        False
-    end.
-  #[local] Instance : CustomIpatFormat "inv_lstate_right" :=
-    " ( %Ψ &
-        #Hη &
-        Hconsumer_au
-      )
-    ".
-
-  #[local] Definition inv_slot γ i slot past : iProp Σ :=
-    match slot with
-    | Nothing =>
-        ⌜past = []⌝
-    | Something v =>
-        history_at γ i (Some v) ∗
-        producers_at γ i Discard ∗
-        lstates_lb γ i Producer
-    | Anything =>
-        consumers_at γ i Discard ∗
-        ( lstates_lb γ i Consumer
-        ∨ producers_at γ i Discard
-        )
-    end.
-  #[local] Instance : CustomIpatFormat "inv_slot_nothing" :=
-    "%Hpast".
-  #[local] Instance : CustomIpatFormat "inv_slot_something" :=
-    " ( #Hhistory_at{_{suff}} &
-        #Hproducers_at{_{suff}} &
-        #Hlstates_lb_producer
-      )
-    ".
-  #[local] Instance : CustomIpatFormat "inv_slot_anything" :=
-    " ( #Hconsumers_at{_{suff}} &
-        { _{suff}
-        ; [ #Hlstates_lb_consumer
-          | #Hproducers_at_
-          ]
-        }
-      )
-    ".
-
-  #[local] Definition inv_inner l γ : iProp Σ :=
-    ∃ front back hist slots vs lstates pasts prophss,
-    l.[front] ↦ #front ∗
-    l.[back] ↦ #back ∗
-    inf_array_model γ.(metadata_data) slots ∗
-    model₂ γ vs ∗
-    ⌜vs = oflatten (drop front hist)⌝ ∗
-    history_auth γ hist ∗
-    ⌜length hist = back⌝ ∗
-    lstates_auth γ lstates ∗
-    ⌜length lstates = front `max` back⌝ ∗
-    wise_prophets_model global_prophet γ.(metadata_prophet) γ.(metadata_prophet_name) pasts prophss ∗
-    producers_auth γ back ∗
-    consumers_auth γ front ∗
-    ( [∗ list] i ↦ lstate ∈ take back lstates,
-      inv_lstate_left γ back i lstate
-    ) ∗
-    ( [∗ list] k ↦ lstate ∈ drop back lstates,
-      inv_lstate_right γ (back + k) lstate
-    ) ∗
-    ( ∀ i,
-      inv_slot γ i (slots i) (pasts i)
-    ).
-  #[local] Instance : CustomIpatFormat "inv_inner" :=
-    " ( %front{} &
-        %back{} &
-        %hist{} &
-        %slots{} &
-        %vs{} &
-        %lstates{} &
-        %pasts{} &
-        %prophss{} &
-        Hl_front &
-        Hl_back &
-        >Hdata_model &
-        Hmodel₂ &
-        >%Hvs{} &
-        Hhistory_auth &
-        >%Hhist{} &
-        Hlstates_auth &
-        >%Hlstates{} &
-        >Hprophet_model &
-        Hproducers_auth &
-        Hconsumers_auth &
-        Hlstates_left &
-        Hlstates_right &
-        Hslots
-      )
-    ".
   Definition inf_mpmc_queue_2_inv t ι : iProp Σ :=
-    ∃ l γ,
-    ⌜t = #l⌝ ∗
-    ⌜ι = γ.(metadata_inv)⌝ ∗
-    meta l nroot γ ∗
-    l.[data] ↦□ γ.(metadata_data) ∗
-    l.[proph] ↦□ #γ.(metadata_prophet) ∗
-    inf_array_inv γ.(metadata_data) ∗
-    inv γ.(metadata_inv) (inv_inner l γ).
+    ∃ 𝑡 γ,
+    ⌜t = #𝑡⌝ ∗
+    meta 𝑡 nroot γ ∗
+    base.inf_mpmc_queue_2_inv 𝑡 γ ι.
   #[local] Instance : CustomIpatFormat "inv" :=
-    " ( %l &
-        %γ &
-        -> &
-        -> &
-        #Hmeta &
-        #Hl_data &
-        #Hl_proph &
-        #Hdata_inv &
-        #Hinv
+    " ( %𝑡{} &
+        %γ{} &
+        {%Heq{};->} &
+        #Hmeta{_{}} &
+        Hinv{_{}}
       )
     ".
 
   Definition inf_mpmc_queue_2_model t vs : iProp Σ :=
-    ∃ l γ,
-    ⌜t = #l⌝ ∗
-    meta l nroot γ ∗
-    model₁ γ vs.
+    ∃ 𝑡 γ,
+    ⌜t = #𝑡⌝ ∗
+    meta 𝑡 nroot γ ∗
+    base.inf_mpmc_queue_2_model γ vs.
   #[local] Instance : CustomIpatFormat "model" :=
-    " ( %l{;_} &
-        %γ{;_} &
-        %Heq{} &
-        Hmeta_{} &
-        Hmodel₁{_{}}
+    " ( %𝑡{} &
+        %γ{} &
+        {%Heq{};->} &
+        Hmeta{_{}} &
+        Hmodel{_{}}
       )
     ".
 
@@ -566,318 +1558,10 @@ Section inf_mpmc_queue_2_G.
     apply _.
   Qed.
 
-  #[local] Instance lstates_at_persistent γ i lstate :
-    Persistent (lstates_at γ i lstate).
-  Proof.
-    apply _.
-  Qed.
-  #[local] Instance lstates_lb_persistent γ i lstate :
-    Persistent (lstates_lb γ i lstate).
-  Proof.
-    apply _.
-  Qed.
-  #[local] Instance producers_at_persistent γ i :
-    Persistent (producers_at γ i Discard).
-  Proof.
-    apply _.
-  Qed.
-  #[local] Instance consumers_at_persistent γ i :
-    Persistent (consumers_at γ i Discard).
-  Proof.
-    apply _.
-  Qed.
-  #[local] Instance consumers_lb_persistent γ i :
-    Persistent (consumers_lb γ i).
-  Proof.
-    apply _.
-  Qed.
-  #[local] Instance inv_slot_persistent γ i slot past :
-    Persistent (inv_slot γ i slot past).
-  Proof.
-    destruct slot; apply _.
-  Qed.
   #[global] Instance inf_mpmc_queue_2_inv_persistent t ι :
     Persistent (inf_mpmc_queue_2_inv t ι).
   Proof.
     apply _.
-  Qed.
-
-  #[local] Lemma model_alloc :
-    ⊢ |==>
-      ∃ γ_model,
-      model₁' γ_model [] ∗
-      model₂' γ_model [].
-  Proof.
-    apply twins_alloc'.
-  Qed.
-  #[local] Lemma model₁_exclusive γ vs1 vs2 :
-    model₁ γ vs1 -∗
-    model₁ γ vs2 -∗
-    False.
-  Proof.
-    apply twins_twin1_exclusive.
-  Qed.
-  #[local] Lemma model_agree γ vs1 vs2 :
-    model₁ γ vs1 -∗
-    model₂ γ vs2 -∗
-    ⌜vs1 = vs2⌝.
-  Proof.
-    apply: twins_agree_L.
-  Qed.
-  #[local] Lemma model_update {γ vs1 vs2} vs :
-    model₁ γ vs1 -∗
-    model₂ γ vs2 ==∗
-      model₁ γ vs ∗
-      model₂ γ vs.
-  Proof.
-    apply twins_update.
-  Qed.
-
-  #[local] Lemma history_alloc :
-    ⊢ |==>
-      ∃ γ_history,
-      history_auth' γ_history [].
-  Proof.
-    apply mono_list_alloc.
-  Qed.
-  #[local] Lemma history_at_lookup γ hist i o :
-    history_auth γ hist -∗
-    history_at γ i o -∗
-    ⌜hist !! i = Some o⌝.
-  Proof.
-    apply mono_list_at_valid.
-  Qed.
-  #[local] Lemma history_at_agree γ i o1 o2 :
-    history_at γ i o1 -∗
-    history_at γ i o2 -∗
-    ⌜o1 = o2⌝.
-  Proof.
-    iIntros "Hat1 Hat2".
-    iDestruct (mono_list_at_agree with "Hat1 Hat2") as %[= <-]. done.
-  Qed.
-  #[local] Lemma history_at_get {γ hist} i o :
-    hist !! i = Some o →
-    history_auth γ hist ⊢
-    history_at γ i o.
-  Proof.
-    apply mono_list_at_get.
-  Qed.
-  #[local] Lemma history_update {γ hist} o :
-    history_auth γ hist ⊢ |==>
-      history_auth γ (hist ++ [o]) ∗
-      history_at γ (length hist) o.
-  Proof.
-    iIntros "Hhistory_auth".
-    iMod (mono_list_update_snoc o with "Hhistory_auth") as "Hhistory_auth".
-    iDestruct (mono_list_at_get with "Hhistory_auth") as "#Hhistory_at".
-    { rewrite list_lookup_middle //. }
-    iSteps.
-  Qed.
-
-  #[local] Lemma lstates_alloc :
-    ⊢ |==>
-      ∃ γ_lstates,
-      lstates_auth' γ_lstates [].
-  Proof.
-    iMod (mono_list_alloc []) as "(%γ_lstates & $)".
-    iSteps.
-  Qed.
-  #[local] Lemma lstates_at_lookup γ lstates i lstate :
-    lstates_auth γ lstates -∗
-    lstates_at γ i lstate -∗
-    ⌜lstates !! i = Some lstate⌝.
-  Proof.
-    iIntros "(:lstates_auth) (:lstates_at)".
-    iDestruct (mono_list_at_valid with "Hauth Hat") as %Hηs_lookup.
-    iDestruct (big_sepL2_lookup_l with "Hηs") as "(%lstate_ & %Hlstates_lookup & Hη_auth_)"; first done.
-    iDestruct (auth_mono_auth_agree_L with "Hη_auth Hη_auth_") as %<-.
-    iSteps.
-  Qed.
-  #[local] Lemma lstates_lb_get {γ lstates} i lstate :
-    lstates !! i = Some lstate →
-    lstates_auth γ lstates -∗
-    lstates_lb γ i (lstate_winner lstate).
-  Proof.
-    iIntros "%Hlstates_lookup (:lstates_auth)".
-    iDestruct (big_sepL2_lookup_r with "Hηs") as "(%η & %Hηs_lookup & Hη_auth)"; first done.
-    iDestruct (auth_mono_lb_get with "Hη_auth") as "Hη_lb".
-    iDestruct (auth_mono_lb_mono with "Hη_lb") as "Hη_lb".
-    { apply lstate_winner_lb. }
-    iDestruct (mono_list_at_get with "Hauth") as "#Hat"; first done.
-    iSteps.
-  Qed.
-  #[local] Lemma lstates_lb_agree γ i lstate1 lstate2 :
-    lstates_lb γ i lstate1 -∗
-    lstates_lb γ i lstate2 -∗
-    ⌜lstate_winner lstate1 = lstate_winner lstate2⌝.
-  Proof.
-    iIntros "(:lstates_lb =1) (:lstates_lb =2)".
-    iDestruct (mono_list_at_agree with "Hat_1 Hat_2") as %<-.
-    iDestruct (auth_mono_lb_agree with "Hη_lb_1 Hη_lb_2") as %(lstate & ->%lsteps_winner & ->%lsteps_winner).
-    iSteps.
-  Qed.
-  #[local] Lemma lstates_update {γ lstates} lstate :
-    lstates_auth γ lstates ⊢ |==>
-      lstates_auth γ (lstates ++ [lstate]) ∗
-      lstates_lb γ (length lstates) (lstate_winner lstate) ∗
-      lstates_at γ (length lstates) lstate.
-  Proof.
-    iIntros "(:lstates_auth)".
-    iMod (auth_mono_alloc _ lstate) as "(%η & Hη_auth)".
-    iMod (auth_mono_auth_persist with "Hη_auth") as "#Hη_auth".
-    iMod (mono_list_update_snoc η with "Hauth") as "Hauth".
-    iDestruct (mono_list_at_get with "Hauth") as "#Hat".
-    { apply list_lookup_middle. done. }
-    iDestruct (auth_mono_lb_get with "Hη_auth") as "#Hη_lb".
-    iDestruct (auth_mono_lb_mono _ (lstate_winner lstate) with "Hη_lb") as "#Hη_lb_winner".
-    { destruct lstate; eauto using rtc, lstep. }
-    iDestruct (big_sepL2_length with "Hηs") as %->.
-    iDestruct (big_sepL2_snoc_2 with "Hηs Hη_auth") as "Hηs".
-    iSteps.
-  Qed.
-
-  #[local] Lemma producers_alloc :
-    ⊢ |==>
-      ∃ γ_producers,
-      producers_auth' γ_producers 0.
-  Proof.
-    iMod (mono_list_alloc []) as "(%γ_producers & $)".
-    iSteps.
-  Qed.
-  #[local] Lemma producers_at_exclusive γ i own :
-    producers_at γ i Own -∗
-    producers_at γ i own -∗
-    False.
-  Proof.
-    iIntros "(:producers_at =1) (:producers_at =2)".
-    iDestruct (mono_list_at_agree with "Hat_1 Hat_2") as %<-.
-    destruct own.
-    - iApply (oneshot_pending_exclusive with "Hη1 Hη2").
-    - iApply (oneshot_pending_shot with "Hη1 Hη2").
-  Qed.
-  #[local] Lemma producers_at_discard γ i :
-    producers_at γ i Own ⊢ |==>
-    producers_at γ i Discard.
-  Proof.
-    iIntros "(:producers_at)".
-    iMod (oneshot_update_shot with "Hη") as "Hη".
-    iSteps.
-  Qed.
-  #[local] Lemma producers_update γ i :
-    producers_auth γ i ⊢ |==>
-      producers_auth γ (S i) ∗
-      producers_at γ i Own.
-  Proof.
-    iIntros "(:producers_auth)".
-    iMod oneshot_alloc as "(%η & Hη_pending)".
-    iMod (mono_list_update_snoc η with "Hauth") as "Hauth".
-    iDestruct (mono_list_at_get with "Hauth") as "#Hat".
-    { apply list_lookup_middle. done. }
-    iSteps. simpl_length/=. iSteps.
-  Qed.
-
-  #[local] Lemma consumers_alloc :
-    ⊢ |==>
-      ∃ γ_consumers,
-      consumers_auth' γ_consumers 0.
-  Proof.
-    iMod (mono_list_alloc []) as "(%γ_consumers & $)".
-    iSteps.
-  Qed.
-  #[local] Lemma consumers_at_exclusive γ i own :
-    consumers_at γ i Own -∗
-    consumers_at γ i own -∗
-    False.
-  Proof.
-    iIntros "(:consumers_at =1) (:consumers_at =2)".
-    iDestruct (mono_list_at_agree with "Hat_1 Hat_2") as %<-.
-    destruct own.
-    - iApply (oneshot_pending_exclusive with "Hη1 Hη2").
-    - iApply (oneshot_pending_shot with "Hη1 Hη2").
-  Qed.
-  #[local] Lemma consumers_at_discard γ i :
-    consumers_at γ i Own ⊢ |==>
-    consumers_at γ i Discard.
-  Proof.
-    iIntros "(:consumers_at)".
-    iMod (oneshot_update_shot with "Hη") as "Hη".
-    iSteps.
-  Qed.
-  #[local] Lemma consumers_lb_valid γ i j :
-    consumers_auth γ i -∗
-    consumers_lb γ j -∗
-    ⌜j ≤ i⌝.
-  Proof.
-    iIntros "(:consumers_auth =1) (:consumers_lb =2)".
-    iDestruct (mono_list_lb_valid with "Hauth1 Hlb2") as %?%prefix_length.
-    iSteps.
-  Qed.
-  #[local] Lemma consumers_lb_le {γ i1} i2 :
-    i2 ≤ i1 →
-    consumers_lb γ i1 ⊢
-    consumers_lb γ i2.
-  Proof.
-    iIntros "% (:consumers_lb)".
-    iDestruct (mono_list_lb_mono (take i2 ηs) with "Hlb") as "$".
-    { apply prefix_take. }
-    simpl_length. iSteps.
-  Qed.
-  #[local] Lemma consumers_lb_get γ i :
-    consumers_auth γ i ⊢
-    consumers_lb γ i.
-  Proof.
-    iIntros "(:consumers_auth)".
-    iDestruct (mono_list_lb_get with "Hauth") as "Hlb".
-    iSteps.
-  Qed.
-  #[local] Lemma consumers_lb_get' {γ i} i' :
-    i' ≤ i →
-    consumers_auth γ i ⊢
-    consumers_lb γ i'.
-  Proof.
-    iIntros "% Hauth".
-    iDestruct (consumers_lb_get with "Hauth") as "Hlb".
-    iDestruct (consumers_lb_le with "Hlb") as "Hlb"; first done.
-    iSteps.
-  Qed.
-  #[local] Lemma consumers_update γ i :
-    consumers_auth γ i ⊢ |==>
-      consumers_auth γ (S i) ∗
-      consumers_at γ i Own.
-  Proof.
-    iIntros "(:consumers_auth)".
-    iMod oneshot_alloc as "(%η & Hη_pending)".
-    iMod (mono_list_update_snoc η with "Hauth") as "Hauth".
-    iDestruct (mono_list_at_get with "Hauth") as "#Hat".
-    { apply list_lookup_middle. done. }
-    iSteps. simpl_length/=. iSteps.
-  Qed.
-
-  Opaque lstates_auth'.
-  Opaque lstates_at.
-  Opaque lstates_lb.
-  Opaque producers_auth'.
-  Opaque producers_at.
-  Opaque consumers_auth'.
-  Opaque consumers_at.
-  Opaque consumers_lb.
-
-  #[local] Lemma winner_exclusive γ i :
-    winner γ i -∗
-    winner γ i -∗
-    False.
-  Proof.
-    iIntros "(:winner =1) (:winner =2)".
-    iDestruct (wise_prophets_full_agree with "Hprophet_full_1 Hprophet_full_2") as %->. simplify.
-    iApply (identifier_model_exclusive with "Hid1 Hid2").
-  Qed.
-
-  #[local] Lemma inv_slot_not_nothing_past {γ i slot past1} past2 :
-    slot ≠ Nothing →
-    inv_slot γ i slot past1 ⊣⊢
-    inv_slot γ i slot past2.
-  Proof.
-    destruct slot; iSteps.
   Qed.
 
   Lemma inf_mpmc_queue_2_model_exclusive t vs1 vs2 :
@@ -887,7 +1571,7 @@ Section inf_mpmc_queue_2_G.
   Proof.
     iIntros "(:model =1) (:model =2)". simplify.
     iDestruct (meta_agree with "Hmeta_1 Hmeta_2") as %->.
-    iApply (model₁_exclusive with "Hmodel₁_1 Hmodel₁_2").
+    iApply (base.inf_mpmc_queue_2_model_exclusive with "Hmodel_1 Hmodel_2").
   Qed.
 
   Lemma inf_mpmc_queue_2_create_spec ι :
@@ -903,35 +1587,10 @@ Section inf_mpmc_queue_2_G.
   Proof.
     iIntros "%Φ _ HΦ".
 
-    wp_rec.
-    wp_apply (wise_prophets_wp_proph global_prophet with "[//]") as "%pid %γ_prophet %prophss Hprophet_model".
-    wp_apply (inf_array_create_spec with "[//]") as (data) "(#Hdata_inv & Hdata_model)".
-    wp_block l as "Hmeta" "(Hl_data & Hl_front & Hl_back & Hl_proph & _)".
-    iMod (pointsto_persist with "Hl_data") as "#Hl_data".
-    iMod (pointsto_persist with "Hl_proph") as "#Hl_proph".
-
-    iMod model_alloc as "(%γ_model & Hmodel₁ & Hmodel₂)".
-    iMod history_alloc as "(%γ_history & Hhistory_auth)".
-    iMod lstates_alloc as "(%γ_lstates & Hlstates_auth)".
-    iMod producers_alloc as "(%γ_producers & Hproducers_auth)".
-    iMod consumers_alloc as "(%γ_consumers & Hconsumers_auth)".
-
-    pose γ := {|
-      metadata_data := data ;
-      metadata_inv := ι ;
-      metadata_prophet := pid ;
-      metadata_prophet_name := γ_prophet ;
-      metadata_model := γ_model ;
-      metadata_history := γ_history ;
-      metadata_lstates := γ_lstates ;
-      metadata_producers := γ_producers ;
-      metadata_consumers := γ_consumers ;
-    |}.
-    iMod (meta_set γ with "Hmeta") as "#Hmeta"; first done.
-
-    iApply "HΦ".
-    iSplitR "Hmodel₁"; last iSteps.
-    iExists l, γ. iSteps. iExists (λ _, Nothing). iSteps. iExists []. iSteps.
+    iApply wp_fupd.
+    wp_apply (base.inf_mpmc_queue_2_create_spec with "[//]") as (𝑡 γ) "(Hmeta & Hinv & Hmodel)".
+    iMod (meta_set γ with "Hmeta"); first done.
+    iSteps.
   Qed.
 
   Lemma inf_mpmc_queue_2_size_spec t ι :
@@ -950,77 +1609,11 @@ Section inf_mpmc_queue_2_G.
   Proof.
     iIntros "%Φ (:inv) HΦ".
 
-    iLöb as "HLöb".
-
-    wp_rec.
-
-    wp_bind (_.{front})%E.
-    iInv "Hinv" as "(:inv_inner =1)".
-    wp_load.
-    iDestruct (consumers_lb_get with "Hconsumers_auth") as "#Hconsumers_lb1".
-    iSplitR "HΦ". { iFrameSteps. }
-    iIntros "!> {%}".
-
-    wp_smart_apply (typed_prophet1_wp_proph local_prophet with "[//]") as (pid proph) "Hproph".
-    wp_pures.
-
-    wp_bind (_.{back})%E.
-    iInv "Hinv" as "(:inv_inner =2)".
-    wp_load.
-    destruct_decide (proph = front1) as -> | Hproph.
-
-    - destruct_decide (front2 = front1) as -> | ?.
-
-      + iMod "HΦ" as "(%vs & (:model) & _ & HΦ)". injection Heq as <-.
-        iDestruct (meta_agree with "Hmeta Hmeta_") as %<-. iClear "Hmeta_".
-        iDestruct (model_agree with "Hmodel₁ Hmodel₂") as %->.
-        iMod ("HΦ" with "[Hmodel₁]") as "HΦ"; first iSteps.
-
-        iSplitR "Hproph HΦ". { iFrameSteps. }
-        iModIntro. clear- Hvs2 Hhist2.
-
-        wp_pures.
-
-        wp_bind (_.{front})%E.
-        iInv "Hinv" as "(:inv_inner =3)".
-        wp_load.
-        iSplitR "Hproph HΦ". { iFrameSteps. }
-        iModIntro. clear -Hvs2 Hhist2.
-
-        wp_smart_apply (typed_prophet1_wp_resolve with "Hproph"); [done.. |].
-        iSteps. iPureIntro.
-        rewrite Hvs2. simpl_length. lia.
-
-      + iDestruct (consumers_lb_valid with "Hconsumers_auth Hconsumers_lb1") as %?.
-        iDestruct (consumers_lb_get with "Hconsumers_auth") as "#Hconsumers_lb2".
-        iSplitR "Hproph HΦ". { iFrameSteps. }
-        iModIntro.
-
-        wp_pures.
-
-        wp_bind (_.{front})%E.
-        iInv "Hinv" as "(:inv_inner =3)".
-        wp_load.
-        iDestruct (consumers_lb_valid with "Hconsumers_auth Hconsumers_lb2") as %?.
-        iSplitR "Hproph HΦ". { iFrameSteps. }
-        iModIntro.
-
-        wp_smart_apply (typed_prophet1_wp_resolve with "Hproph"); [done.. |].
-        iSteps.
-
-    - iSplitR "Hproph HΦ". { iFrameSteps. }
-      iModIntro. clear- Hproph.
-
-      wp_pures.
-
-      wp_bind (_.{front})%E.
-      iInv "Hinv" as "(:inv_inner =3)".
-      wp_load.
-      iSplitR "Hproph HΦ". { iFrameSteps. }
-      iModIntro. clear- Hproph.
-
-      wp_smart_apply (typed_prophet1_wp_resolve with "Hproph"); [done.. |].
-      iSteps.
+    awp_apply (base.inf_mpmc_queue_2_size_spec with "[$]").
+    { iApply (aacc_aupd_commit with "HΦ"); first done. iIntros "%vs (:model =1)". simplify.
+      iDestruct (meta_agree with "Hmeta Hmeta_1") as %<-. iClear "Hmeta_1".
+      iAaccIntro with "Hmodel_1"; iSteps.
+    }
   Qed.
 
   Lemma inf_mpmc_queue_2_is_empty_spec t ι :
@@ -1037,15 +1630,13 @@ Section inf_mpmc_queue_2_G.
       ⌜if b then vs = [] else True⌝
     >>>.
   Proof.
-    iIntros "%Φ #Hinv HΦ".
+    iIntros "%Φ (:inv) HΦ".
 
-    wp_rec.
-
-    awp_apply (inf_mpmc_queue_2_size_spec with "Hinv").
-    iApply (aacc_aupd_commit with "HΦ"); first done. iIntros "%vs Hmodel".
-    iAaccIntro with "Hmodel"; iSteps. iPureIntro.
-    case_bool_decide as Hlength; last done.
-    apply nil_length_inv. lia.
+    awp_apply (base.inf_mpmc_queue_2_is_empty_spec with "[$]").
+    { iApply (aacc_aupd_commit with "HΦ"); first done. iIntros "%vs (:model =1)". simplify.
+      iDestruct (meta_agree with "Hmeta Hmeta_1") as %<-. iClear "Hmeta_1".
+      iAaccIntro with "Hmodel_1"; iSteps.
+    }
   Qed.
 
   Lemma inf_mpmc_queue_2_push_spec t ι v :
@@ -1063,233 +1654,11 @@ Section inf_mpmc_queue_2_G.
   Proof.
     iIntros "%Φ (:inv) HΦ".
 
-    iLöb as "HLöb".
-
-    wp_rec.
-    wp_smart_apply (wp_id with "[//]") as (id) "Hid".
-    wp_pures.
-
-    wp_bind (FAA _ _).
-    iInv "Hinv" as "(:inv_inner =1)".
-    wp_faa.
-    iMod (producers_update with "Hproducers_auth") as "(Hproducers_auth & Hproducers_at)".
-    iDestruct (wise_prophets_full_get' _ back1 with "Hprophet_model") as "(%prophs & #Hprophet_full)".
-    destruct_decide (front1 ≤ back1) as Hfirst | Hlast.
-
-    - rewrite Nat.max_r // in Hlstates1.
-      rewrite firstn_all2; first lia.
-
-      destruct_decide (head prophs = Some id) as Hwinner | Hloser.
-
-      + iMod (history_update (Some v) with "Hhistory_auth") as "(Hhistory_auth & #Hhistory_at)". rewrite Hhist1.
-        iMod (lstates_update ProducerProducer with "Hlstates_auth") as "(Hlstates_auth & #Hlstates_lb & _)". rewrite Hlstates1.
-        iDestruct (big_sepL_snoc_2 ProducerProducer with "Hlstates_left [Hid]") as "Hlstates_left".
-        { rewrite Hlstates1. iSteps. }
-
-        iMod "HΦ" as "(%vs & (:model) & _ & HΦ)". injection Heq as <-.
-        iDestruct (meta_agree with "Hmeta Hmeta_") as %<-. iClear "Hmeta_".
-        iDestruct (model_agree with "Hmodel₁ Hmodel₂") as %<-.
-        iMod (model_update (vs ++ [v]) with "Hmodel₁ Hmodel₂") as "(Hmodel₁ & Hmodel₂)".
-        iMod ("HΦ" with "[Hmodel₁] [//]") as "HΦ"; first iFrameSteps.
-
-        iSplitR "Hproducers_at HΦ".
-        { iFrame.
-          rewrite firstn_all2. { simpl_length/=. lia. }
-          rewrite (skipn_all2 (n := S back1)).
-          { simpl_length/=. lia. }
-          iFrameSteps; iPureIntro.
-          - rewrite drop_app_le; first lia.
-            rewrite oflatten_snoc_Some Hvs1 //.
-          - simpl_length/=. lia.
-          - simpl_length/=. lia.
-        }
-        iModIntro. clear- Hwinner.
-
-        do 2 wp_load.
-
-        wp_apply (inf_array_cas_resolve_spec with "Hdata_inv"); first lia.
-        iMod (inv_acc with "Hinv") as "((:inv_inner =2) & Hclose1)"; first done.
-        iStep. iIntros "%e %b % % %Hslots2 Hdata_model".
-        rewrite Nat2Z.id in Hslots2 |- *.
-        wp_apply (wise_prophets_wp_resolve' with "Hprophet_model"); [done.. |].
-        wp_pures.
-        iIntros "!> %prophs2 %Hprophss2 Hprophet_model".
-        destruct b; last first.
-        { iDestruct ("Hslots" $! back1) as "Hslot".
-          destruct (slots2 back1).
-          - exfalso. done.
-          - iDestruct "Hslot" as "(:inv_slot_anything)".
-            + iDestruct (lstates_lb_agree with "Hlstates_lb Hlstates_lb_consumer") as %[=].
-            + iDestruct (producers_at_exclusive with "Hproducers_at Hproducers_at_") as %[].
-          - iDestruct "Hslot" as "(:inv_slot_something suff=)".
-            iDestruct (producers_at_exclusive with "Hproducers_at Hproducers_at_") as %[].
-        }
-        iMod (producers_at_discard with "Hproducers_at") as "#Hproducers_at".
-        iMod ("Hclose1" with "[- HΦ]") as "_".
-        { rewrite -(fn_compose_insert _ _ _ (Something v)).
-          iFrameSteps.
-          rewrite function.fn_lookup_insert. case_decide.
-          - subst. iSteps.
-          - rewrite fn_lookup_alter_ne //.
-        }
-        iSteps.
-
-      + iMod (history_update None with "Hhistory_auth") as "(Hhistory_auth & #Hhistory_at)". rewrite Hhist1.
-        iMod (lstates_update ProducerConsumer with "Hlstates_auth") as "(Hlstates_auth & Hlstates_lb & _)".
-        iDestruct (big_sepL_snoc_2 ProducerConsumer with "Hlstates_left []") as "Hlstates_left".
-        { rewrite Hlstates1 //. }
-        iSplitR "HΦ".
-        { iFrame.
-          rewrite firstn_all2. { simpl_length/=. lia. }
-          rewrite (skipn_all2 (n := S back1)).
-          { simpl_length/=. lia. }
-          iFrameSteps; iPureIntro.
-          - rewrite drop_app_le; first lia.
-            rewrite oflatten_snoc_None Hvs1 //.
-          - simpl_length/=. lia.
-          - simpl_length/=. lia.
-        }
-        iModIntro. clear- Hloser.
-
-        do 2 wp_load.
-
-        wp_apply (inf_array_cas_resolve_spec with "Hdata_inv"); first lia.
-        iMod (inv_acc with "Hinv") as "((:inv_inner =2) & Hclose1)"; first done.
-        iStep. iIntros "%e %b % % %Hslots2 Hdata_model".
-        rewrite Nat2Z.id in Hslots2 |- *.
-        wp_apply (wise_prophets_wp_resolve' with "Hprophet_model"); [done.. |].
-        wp_pures.
-        iIntros "!> %prophs2 %Hprophss2 Hprophet_model".
-        destruct b.
-        { iDestruct ("Hslots" $! back1) as "Hslot".
-          destruct (slots2 back1).
-          - iDestruct "Hslot" as "(:inv_slot_nothing)".
-            iDestruct (wise_prophets_full_valid with "Hprophet_model Hprophet_full") as %Hprophs.
-            exfalso.
-            rewrite fn_lookup_alter Hpast /= in Hprophs. naive_solver.
-          - exfalso. done.
-          - exfalso. done.
-        }
-        iMod ("Hclose1" with "[- HΦ]") as "_".
-        { iFrameSteps.
-          rewrite function.fn_lookup_alter. case_decide; last done.
-          subst. rewrite inv_slot_not_nothing_past //.
-          intros Heq. rewrite Heq // in Hslots2.
-        }
-        iSteps.
-
-    - rewrite drop_ge /= in Hvs1; first lia. subst vs1.
-      rewrite Nat.max_l in Hlstates1; first lia.
-      iDestruct (consumers_lb_get' (S back1) with "Hconsumers_auth") as "#Hconsumers_lb"; first lia.
-      destruct (lookup_lt_is_Some_2 lstates1 back1) as (lstate & Hlstates_lookup); first lia.
-      iDestruct (lstates_lb_get with "Hlstates_auth") as "#Hlstates_lb"; first done.
-      erewrite drop_S; last done.
-      iDestruct "Hlstates_right" as "(Hlstate & Hlstates_right)".
-
-      destruct lstate as [| | | | η |].
-      all: try iDestruct "Hlstate" as %[].
-
-      + iDestruct "Hlstate" as "(:inv_lstate_right)".
-
-        iMod "HΦ" as "(%vs & (:model) & _ & HΦ)". injection Heq as <-.
-        iDestruct (meta_agree with "Hmeta Hmeta_") as %<-. iClear "Hmeta_".
-        iDestruct (model_agree with "Hmodel₁ Hmodel₂") as %->.
-        iMod (model_update [v] with "Hmodel₁ Hmodel₂") as "(Hmodel₁ & Hmodel₂)".
-        iMod ("HΦ" with "[Hmodel₁] [//]") as "HΦ"; first iFrameSteps.
-
-        iMod "Hconsumer_au" as "(%vs & Hmodel₁ & _ & HΨ)".
-        iDestruct (model_agree with "Hmodel₁ Hmodel₂") as %->.
-        iMod (model_update [] with "Hmodel₁ Hmodel₂") as "(Hmodel₁ & Hmodel₂)".
-        iMod ("HΨ" with "[$Hmodel₁ //]") as "HΨ".
-
-        iMod (history_update (Some v) with "Hhistory_auth") as "(Hhistory_auth & #Hhistory_lb)". rewrite Hhist1.
-        iDestruct (big_sepL_snoc_2 (ConsumerProducer η) with "Hlstates_left [HΨ]") as "Hlstates_left".
-        { rewrite /= length_take Nat.min_l; first lia. iSteps. }
-        iSplitR "Hproducers_at HΦ".
-        { rewrite -take_S_r //.
-          setoid_rewrite Nat.add_succ_r.
-          iFrameSteps; iPureIntro.
-          - rewrite drop_ge //. { simpl_length/=. lia. }
-          - simpl_length/=. lia.
-        }
-        iIntros "!> {%}".
-
-        do 2 wp_load.
-
-        wp_apply (inf_array_cas_resolve_spec with "Hdata_inv"); first lia.
-        iMod (inv_acc with "Hinv") as "((:inv_inner =2) & Hclose1)"; first done.
-        iStep. iIntros "%e %b % % %Hslots2 Hdata_model".
-        rewrite Nat2Z.id in Hslots2 |- *.
-        wp_apply (wise_prophets_wp_resolve' with "Hprophet_model"); [done.. |].
-        wp_pures.
-        iIntros "!> %prophs2 %Hprophss2 Hprophet_model".
-        destruct b; last first.
-        { iDestruct ("Hslots" $! back1) as "Hslot".
-          destruct (slots2 back1).
-          - iDestruct "Hslot" as "(:inv_slot_nothing)".
-            iDestruct (wise_prophets_full_valid with "Hprophet_model Hprophet_full") as %Hprophs.
-            exfalso.
-            rewrite fn_lookup_alter Hpast /= in Hprophs. naive_solver.
-          - iDestruct "Hslot" as "(:inv_slot_anything)".
-            + iDestruct (lstates_lb_agree with "Hlstates_lb Hlstates_lb_consumer") as %[=].
-            + iDestruct (producers_at_exclusive with "Hproducers_at Hproducers_at_") as %[].
-          - iDestruct "Hslot" as "(:inv_slot_something suff=)".
-            iDestruct (producers_at_exclusive with "Hproducers_at Hproducers_at_") as %[].
-        }
-        iMod (producers_at_discard with "Hproducers_at") as "#Hproducers_at".
-        iMod ("Hclose1" with "[- HΦ]") as "_".
-        { rewrite -(fn_compose_insert _ _ _ (Something v)).
-          iFrameSteps.
-          rewrite function.fn_lookup_insert. case_decide.
-          - subst. iSteps.
-          - rewrite fn_lookup_alter_ne //.
-        }
-        iSteps.
-
-      + iAssert ⌜head prophs ≠ Some id⌝%I as %Hloser.
-        { iIntros (Hwinner).
-          iEval (rewrite /= Nat.add_0_r) in "Hlstate".
-          iDestruct (winner_exclusive with "Hlstate [Hid]") as %[]; first iSteps.
-        }
-
-        iMod (history_update None with "Hhistory_auth") as "(Hhistory_auth & _)".
-        iDestruct (big_sepL_snoc_2 ConsumerConsumer with "Hlstates_left []") as "Hlstates_left".
-        { rewrite /= length_take Nat.min_l; first lia. iSteps. }
-        iSplitR "HΦ".
-        { rewrite -take_S_r //.
-          setoid_rewrite Nat.add_succ_r.
-          iFrameSteps; iPureIntro.
-          - rewrite drop_ge //. { simpl_length/=. lia. }
-          - simpl_length/=. lia.
-        }
-        iModIntro. clear- Hloser.
-
-        do 2 wp_load.
-
-        wp_apply (inf_array_cas_resolve_spec with "Hdata_inv"); first lia.
-        iMod (inv_acc with "Hinv") as "((:inv_inner =2) & Hclose1)"; first done.
-        iStep. iIntros "%e %b % % %Hslots2 Hdata_model".
-        rewrite Nat2Z.id in Hslots2 |- *.
-        wp_apply (wise_prophets_wp_resolve' with "Hprophet_model"); [done.. |].
-        wp_pures.
-        iIntros "!> %prophs2 %Hprophss2 Hprophet_model".
-        destruct b.
-        { iDestruct ("Hslots" $! back1) as "Hslot".
-          destruct (slots2 back1).
-          - iDestruct "Hslot" as "(:inv_slot_nothing)".
-            iDestruct (wise_prophets_full_valid with "Hprophet_model Hprophet_full") as %Hprophs.
-            exfalso.
-            rewrite fn_lookup_alter Hpast /= in Hprophs. naive_solver.
-          - exfalso. done.
-          - exfalso. done.
-        }
-        iMod ("Hclose1" with "[- HΦ]") as "_".
-        { iFrameSteps.
-          rewrite function.fn_lookup_alter. case_decide; last done.
-          subst. rewrite inv_slot_not_nothing_past //.
-          intros Heq. rewrite Heq // in Hslots2.
-        }
-        iSteps.
+    awp_apply (base.inf_mpmc_queue_2_push_spec with "[$]").
+    { iApply (aacc_aupd_commit with "HΦ"); first done. iIntros "%vs (:model =1)". simplify.
+      iDestruct (meta_agree with "Hmeta Hmeta_1") as %<-. iClear "Hmeta_1".
+      iAaccIntro with "Hmodel_1"; iSteps.
+    }
   Qed.
 
   Lemma inf_mpmc_queue_2_pop_spec t ι :
@@ -1309,232 +1678,13 @@ Section inf_mpmc_queue_2_G.
   Proof.
     iIntros "%Φ (:inv) HΦ".
 
-    iLöb as "HLöb".
-
-    wp_rec.
-    wp_smart_apply (wp_id with "[//]") as (id) "Hid".
-    wp_pures.
-
-    wp_bind (FAA _ _).
-    iInv "Hinv" as "(:inv_inner =1)".
-    wp_faa.
-    iDestruct (wise_prophets_full_get' _ front1 with "Hprophet_model") as "(%prophs & #Hprophet_full)".
-    destruct_decide (back1 ≤ front1) as Hfirst | Hlast.
-
-    - rewrite drop_ge /= in Hvs1; first lia. subst vs1.
-      rewrite Nat.max_l // in Hlstates1.
-
-      iMod (consumers_update with "Hconsumers_auth") as "(Hconsumers_auth & Hconsumers_at)".
-
-      destruct_decide (head prophs = Some id) as Hwinner | Hloser.
-
-      + iMod (lstates_update ConsumerConsumer with "Hlstates_auth") as "(Hlstates_auth & #Hlstates_lb & _)". rewrite Hlstates1.
-        iDestruct (big_sepL_snoc_2 ConsumerConsumer with "Hlstates_right [Hid]") as "Hlstates_right".
-        { rewrite length_drop Hlstates1 -Nat.le_add_sub; first lia.
-          iSteps.
-        }
-
-        iSplitR "Hconsumers_at HΦ".
-        { iFrame.
-          rewrite (drop_ge hist1); first lia.
-          rewrite take_app_le; first lia.
-          rewrite drop_app_le; first lia.
-          iFrameSteps. iPureIntro.
-          simpl_length/=. lia.
-        }
-        iModIntro. clear- Hwinner.
-
-        do 2 wp_load.
-
-        wp_apply (inf_array_xchg_resolve_spec with "Hdata_inv"); first lia.
-        iMod (inv_acc with "Hinv") as "((:inv_inner =2) & Hclose1)"; first done.
-        iStep. iIntros "%e % % Hdata_model".
-        rewrite Nat2Z.id.
-        wp_apply (wise_prophets_wp_resolve' with "Hprophet_model"); [done.. |].
-        wp_pures.
-        iIntros "!> %prophs2 %Hprophss2 Hprophet_model".
-        iDestruct (bi.forall_elim front1 with "Hslots") as "#-#Hslot".
-        destruct (slots2 front1); first last.
-        { iDestruct "Hslot" as "(:inv_slot_something)".
-          iDestruct (lstates_lb_agree with "Hlstates_lb Hlstates_lb_producer") as %[=].
-        } {
-          iDestruct "Hslot" as "(:inv_slot_anything suff=)".
-          iDestruct (consumers_at_exclusive with "Hconsumers_at Hconsumers_at_") as %[].
-        }
-        iMod (consumers_at_discard with "Hconsumers_at") as "#Hconsumers_at".
-        iMod ("Hclose1" with "[- HΦ]") as "_".
-        { rewrite -(fn_compose_insert _ _ _ Anything).
-          iFrameSteps.
-          rewrite function.fn_lookup_insert. case_decide.
-          - subst. iSteps.
-          - rewrite fn_lookup_alter_ne //.
-        }
-        iSteps.
-
-      + iMod (saved_pred_alloc Φ) as "(%η & #Hη)".
-        iMod (lstates_update (ConsumerProducer η) with "Hlstates_auth") as "(Hlstates_auth & _ & #Hlstates_at)". rewrite Hlstates1.
-        iDestruct (big_sepL_snoc_2 (ConsumerProducer η) with "Hlstates_right [HΦ]") as "Hlstates_right".
-        { iSteps.
-          rewrite /consumer_au. iAuIntro.
-          iApply (aacc_aupd_commit with "HΦ"); first done. iIntros "%vs (:model)". injection Heq as <-.
-          iDestruct (meta_agree with "Hmeta Hmeta_") as %<-. iClear "Hmeta_".
-          iAaccIntro with "Hmodel₁"; iSteps.
-        }
-
-        iSplitR "Hconsumers_at".
-        { iFrame.
-          rewrite (drop_ge hist1); first lia.
-          rewrite take_app_le; first lia.
-          rewrite drop_app_le; first lia.
-          iFrameSteps. iPureIntro.
-          simpl_length/=. lia.
-        }
-        iModIntro. clear- Hloser.
-
-        do 2 wp_load.
-
-        wp_apply (inf_array_xchg_resolve_spec with "Hdata_inv"); first lia.
-        iMod (inv_acc with "Hinv") as "((:inv_inner =2) & Hclose1)"; first done.
-        iStep. iIntros "%e % % Hdata_model".
-        rewrite Nat2Z.id.
-        wp_apply (wise_prophets_wp_resolve' with "Hprophet_model"); [done.. |].
-        wp_pures.
-        iIntros "!> %prophs2 %Hprophss2 Hprophet_model".
-        iDestruct (bi.forall_elim front1 with "Hslots") as "#-#Hslot".
-        destruct (slots2 front1) as [| | v].
-        { iDestruct "Hslot" as "(:inv_slot_nothing)".
-          iDestruct (wise_prophets_full_valid with "Hprophet_model Hprophet_full") as %Hprophs.
-          exfalso.
-          rewrite fn_lookup_alter Hpast /= in Hprophs. naive_solver.
-        } {
-          iDestruct "Hslot" as "(:inv_slot_anything suff=)".
-          iDestruct (consumers_at_exclusive with "Hconsumers_at Hconsumers_at_") as %[].
-        }
-        iDestruct "Hslot" as "(:inv_slot_something)".
-
-        iDestruct (lstates_at_lookup with "Hlstates_auth Hlstates_at") as %Hlstates2_lookup.
-        iDestruct (history_at_lookup with "Hhistory_auth Hhistory_at") as %?%lookup_lt_Some.
-        iDestruct (big_sepL_lookup_acc with "Hlstates_left") as "(Hlstate & Hlstates_left)".
-        { rewrite lookup_take_Some. naive_solver. }
-        iDestruct "Hlstate" as "(:inv_lstate_left_consumer suff=)".
-        iDestruct (history_at_agree with "Hhistory_at Hhistory_at_") as %[= <-].
-        iDestruct (saved_pred_agree v with "Hη Hη_") as "#Heq".
-        iDestruct "HΨ" as "[HΦ | Hconsumers_at_]"; last first.
-        { iDestruct (consumers_at_exclusive with "Hconsumers_at Hconsumers_at_") as %[]. }
-
-        iMod (consumers_at_discard with "Hconsumers_at") as "#Hconsumers_at".
-        iMod ("Hclose1" with "[- HΦ]") as "_".
-        { rewrite -(fn_compose_insert _ _ _ Anything).
-          iFrameSteps.
-          rewrite function.fn_lookup_insert. case_decide.
-          - subst. iSteps.
-          - rewrite fn_lookup_alter_ne //.
-        }
-        iIntros "!> {%}".
-
-        wp_pures.
-        iRewrite "Heq". iSteps.
-
-    - rewrite Nat.max_r in Hlstates1; first lia.
-      destruct (lookup_lt_is_Some_2 lstates1 front1) as (lstate & Hlstates_lookup); first lia.
-      iDestruct (big_sepL_lookup_acc with "Hlstates_left") as "(Hlstate & Hlstates_left)".
-      { rewrite lookup_take_Some. naive_solver lia. }
-      destruct lstate.
-      all: try iDestruct "Hlstate" as %[].
-      1,2: iMod (consumers_update with "Hconsumers_auth") as "(Hconsumers_auth & Hconsumers_at)".
-
-      + iDestruct "Hlstate" as "(:inv_lstate_left_producer)".
-        iDestruct (history_at_lookup with "Hhistory_auth Hhistory_at") as %Hhist1_lookup.
-        erewrite drop_S, oflatten_cons_Some in Hvs1; last done.
-
-        iAssert ⌜head prophs ≠ Some id⌝%I as %Hloser.
-        { iIntros (Hwinner).
-          iDestruct (winner_exclusive with "Hwinner [Hid]") as %[]; first iSteps.
-        }
-
-        iMod "HΦ" as "(%vs & (:model) & _ & HΦ)". injection Heq as <-.
-        iDestruct (meta_agree with "Hmeta Hmeta_") as %<-. iClear "Hmeta_".
-        iDestruct (model_agree with "Hmodel₁ Hmodel₂") as %<-.
-        iMod (model_update with "Hmodel₁ Hmodel₂") as "(Hmodel₁ & Hmodel₂)".
-        iMod ("HΦ" with "[Hmodel₁] [//]") as "HΦ"; first iSteps.
-
-        iSplitR "Hconsumers_at HΦ". { iFrameSteps. }
-        iModIntro. clear- Hloser.
-
-        do 2 wp_load.
-
-        wp_apply (inf_array_xchg_resolve_spec with "Hdata_inv"); first lia.
-        iMod (inv_acc with "Hinv") as "((:inv_inner =2) & Hclose1)"; first done.
-        iStep. iIntros "%e % % Hdata_model".
-        rewrite Nat2Z.id.
-        wp_apply (wise_prophets_wp_resolve' with "Hprophet_model"); [done.. |].
-        wp_pures.
-        iIntros "!> %prophs2 %Hprophss2 Hprophet_model".
-        iDestruct (bi.forall_elim front1 with "Hslots") as "#-#Hslot".
-        destruct (slots2 front1) as [| | v_].
-        { iDestruct "Hslot" as "(:inv_slot_nothing)".
-          iDestruct (wise_prophets_full_valid with "Hprophet_model Hprophet_full") as %Hprophs.
-          exfalso.
-          rewrite fn_lookup_alter Hpast /= in Hprophs. naive_solver.
-        } {
-          iDestruct "Hslot" as "(:inv_slot_anything suff=)".
-          iDestruct (consumers_at_exclusive with "Hconsumers_at Hconsumers_at_") as %[].
-        }
-        iDestruct "Hslot" as "(:inv_slot_something suff=)".
-        iDestruct (history_at_agree with "Hhistory_at Hhistory_at_") as %[= <-].
-        iMod (consumers_at_discard with "Hconsumers_at") as "#Hconsumers_at".
-        iMod ("Hclose1" with "[- HΦ]") as "_".
-        { rewrite -(fn_compose_insert _ _ _ Anything).
-          iFrameSteps.
-          rewrite function.fn_lookup_insert. case_decide.
-          - subst. iSteps.
-          - rewrite fn_lookup_alter_ne //.
-        }
-        iSteps.
-
-      + iDestruct (history_at_lookup with "Hhistory_auth Hlstate") as %Hhist1_lookup.
-        erewrite drop_S, oflatten_cons_None in Hvs1; last done.
-        iDestruct (lstates_lb_get with "Hlstates_auth") as "#Hlstates_lb"; first done.
-
-        iSplitR "Hconsumers_at HΦ". { iFrameSteps. }
-        iIntros "!> {%}".
-
-        do 2 wp_load.
-
-        wp_apply (inf_array_xchg_resolve_spec with "Hdata_inv"); first lia.
-        iMod (inv_acc with "Hinv") as "((:inv_inner =2) & Hclose1)"; first done.
-        iStep. iIntros "%e % % Hdata_model".
-        rewrite Nat2Z.id.
-        wp_apply (wise_prophets_wp_resolve' with "Hprophet_model"); [done.. |].
-        wp_pures.
-        iIntros "!> %prophs2 %Hprophss2 Hprophet_model".
-        iDestruct (bi.forall_elim front1 with "Hslots") as "#-#Hslot".
-        destruct (slots2 front1) as [| | v]; first last.
-        { iDestruct "Hslot" as "(:inv_slot_something)".
-          iDestruct (lstates_lb_agree with "Hlstates_lb Hlstates_lb_producer") as %[=].
-        } {
-          iDestruct "Hslot" as "(:inv_slot_anything suff=)".
-          iDestruct (consumers_at_exclusive with "Hconsumers_at Hconsumers_at_") as %[].
-        }
-        iMod (consumers_at_discard with "Hconsumers_at") as "#Hconsumers_at".
-        iMod ("Hclose1" with "[- HΦ]") as "_".
-        { rewrite -(fn_compose_insert _ _ _ Anything).
-          iFrameSteps.
-          rewrite function.fn_lookup_insert. case_decide.
-          - subst. iSteps.
-          - rewrite fn_lookup_alter_ne //.
-        }
-        iSteps.
-
-      + iDestruct "Hlstate" as "(:inv_lstate_left_consumer)".
-        iDestruct (consumers_lb_valid with "Hconsumers_auth Hconsumers_lb") as %?. lia.
-
-      + iDestruct (consumers_lb_valid with "Hconsumers_auth Hlstate") as %?. lia.
+    awp_apply (base.inf_mpmc_queue_2_pop_spec with "[$]").
+    { iApply (aacc_aupd_commit with "HΦ"); first done. iIntros "%vs (:model =1)". simplify.
+      iDestruct (meta_agree with "Hmeta Hmeta_1") as %<-. iClear "Hmeta_1".
+      iAaccIntro with "Hmodel_1"; iSteps.
+    }
   Qed.
 End inf_mpmc_queue_2_G.
-
-From zoo_saturn Require
-  inf_mpmc_queue_2__opaque.
 
 #[global] Opaque inf_mpmc_queue_2_inv.
 #[global] Opaque inf_mpmc_queue_2_model.
